upload new models for sync changes

driver_model/driver_checkScript.sml
@@ -5,155 +5,123 @@ open driver_stateTheory board_memTheory;
 (* Driver checks the reply from the SPI controller for a read request *)
 val _ = new_theory "driver_check";
 
-(* INIT_CHECK_ENABLE: driver_state -> bool *)
-val INIT_CHECK_ENABLE_def = Define `
-INIT_CHECK_ENABLE (dr:driver_state) =
-(dr.dr_init.state = dr_init_check_rep)`
+(* DR_TAU_ENABLE: driver_state -> bool *)
+val DR_TAU_ENABLE_def = Define `
+DR_TAU_ENABLE (dr:driver_state) =
+(dr.state = dr_init_check_rep \/
+dr.state = dr_tx_check_txs \/
+dr.state = dr_tx_check_eot \/
+dr.state = dr_rx_check_rxs \/
+dr.state = dr_rx_fetch_data \/
+dr.state = dr_xfer_check_txs \/
+dr.state = dr_xfer_check_rxs \/
+dr.state = dr_xfer_fetch_dataI)`
 
-(* TX_CHECK_ENABLE: driver_state -> bool *)
-val TX_CHECK_ENABLE_def = Define `
-TX_CHECK_ENABLE (dr:driver_state) =
-((dr.dr_tx.state = dr_tx_check_txs) \/
-(dr.dr_tx.state = dr_tx_check_eot))`
-
-(* RX_CHECK_ENABLE: driver_state -> bool *)
-val RX_CHECK_ENABLE_def = Define `
-RX_CHECK_ENABLE (dr:driver_state) =
-((dr.dr_rx.state = dr_rx_check_rxs) \/
-(dr.dr_rx.state = dr_rx_fetch_data))`
-
-(* XFER_CHECK_ENABLE: driver_state -> bool *)
-val XFER_CHECK_ENABLE_def = Define `
-XFER_CHECK_ENABLE (dr:driver_state) =
-((dr.dr_xfer.state = dr_xfer_check_txs) \/
-(dr.dr_xfer.state = dr_xfer_check_rxs) \/
-(dr.dr_xfer.state = dr_xfer_fetch_dataI))`
-
-(* CHECK_ENABLE: driver_state -> bool *)
-val CHECK_ENABLE_def = Define `
-CHECK_ENABLE (dr:driver_state) =
-((INIT_CHECK_ENABLE dr) \/ (TX_CHECK_ENABLE dr) \/ 
-(RX_CHECK_ENABLE dr) \/ (XFER_CHECK_ENABLE dr))`
-
-(* dr_check_sysstatus:driver_state -> word32 -> driver_state *)
+(* dr_check_sysstatus: driver_state -> word32 -> driver_state *)
 val dr_check_sysstatus_def = Define `
 dr_check_sysstatus (dr:driver_state) (rep_v:word32) =
 let v = (0 >< 0) rep_v:word1 in
-case dr.dr_init.state of
-  | dr_init_pre => dr
-  | dr_init_idle => dr
-  | dr_init_read_req => dr
-  | dr_init_check_rep => if v = 1w 
-    then dr with <| dr_init := dr.dr_init with state := dr_init_setting;
-    dr_tx := dr.dr_tx with state := dr_tx_not_ready;
-    dr_rx := dr.dr_rx with state := dr_rx_not_ready;
-    dr_xfer := dr.dr_xfer with state := dr_xfer_not_ready |>
-    else dr with dr_init := dr.dr_init with state := dr_init_read_req
-  | dr_init_setting => dr
-  | dr_init_done => dr`
+if v = 1w (* RESET is done *) 
+then dr with state := dr_init_setting
+else dr with state := dr_init_read_req`
 
 (* dr_check_tx_ch0stat:driver_state -> word32 -> driver_state *)
 val dr_check_tx_ch0stat_def = Define `
 dr_check_tx_ch0stat (dr:driver_state) (rep_v:word32) =
 let v1 = (1 >< 1) rep_v:word1 and
     v2 = (2 >< 2) rep_v:word1 in
-case dr.dr_tx.state of
-  | dr_tx_not_ready => dr
-  | dr_tx_pre => dr
-  | dr_tx_idle => dr
-  | dr_tx_conf_issued => dr 
-  | dr_tx_read_txs => dr
-  | dr_tx_check_txs => if v1 = 1w
-    then dr with dr_tx := dr.dr_tx with state := dr_tx_write_data
-    else dr with dr_tx := dr.dr_tx with state := dr_tx_read_txs
-  | dr_tx_write_data => dr
-  | dr_tx_read_eot => dr
-  | dr_tx_check_eot => if (v1 = 1w) /\ (v2 = 1w)
-    then dr with dr_tx := dr.dr_tx with state := dr_tx_issue_disable
-    else dr with dr_tx := dr.dr_tx with state := dr_tx_read_eot
-  | dr_tx_issue_disable => dr 
-  | dr_tx_reset_conf => dr`
+if (dr.state = dr_tx_check_txs) /\ (v1 = 1w) then 
+dr with state := dr_tx_write_data
+else if (dr.state = dr_tx_check_txs) /\ (v1 = 0w) then
+dr with state := dr_tx_read_txs
+else if (dr.state = dr_tx_check_eot) /\ (v2 = 1w) then
+dr with state := dr_tx_issue_disable
+else if (dr.state = dr_tx_check_eot) /\ (v2 = 0w) then
+dr with state := dr_tx_read_eot
+else dr with dr_err := T`
 
 (* dr_check_rx_ch0stat:driver_state -> word32 -> driver_state *)
 val dr_check_rx_ch0stat_def = Define `
 dr_check_rx_ch0stat (dr:driver_state) (rep_v:word32) =
 let v = (0 >< 0) rep_v:word1 in
-case dr.dr_rx.state of
-  | dr_rx_idle => dr 
-  | dr_rx_conf_issued => dr
-  | dr_rx_read_rxs => dr
-  | dr_rx_check_rxs => if v = 1w
-    then dr with dr_rx := dr.dr_rx with state := dr_rx_read_rx0
-    else dr with dr_rx := dr.dr_rx with state := dr_rx_read_rxs
-  | dr_rx_read_rx0 => dr
-  | dr_rx_fetch_data => dr
-  | dr_rx_issue_diable => dr
-  | dr_rx_reset_conf => dr`
+if v = 1w
+then dr with state := dr_rx_read_rx0
+else dr with state := dr_rx_read_rxs`
 
 (* dr_check_xfer_ch0stat:driver_state -> word32 -> driver_state *)
 val dr_check_xfer_ch0stat_def = Define `
 dr_check_xfer_ch0stat (dr:driver_state) (rep_v:word32) =
 let rxs = (0 >< 0) rep_v:word1 and
     txs = (1 >< 1) rep_v:word1 in
-case dr.dr_xfer.state of
-  | dr_xfer_idle => dr
-  | dr_xfer_conf_issued => dr
-  | dr_xfer_read_txs => dr
-  | dr_xfer_check_txs => if txs = 1w 
-    then dr with dr_xfer := dr.dr_xfer with state := dr_xfer_write_dataO
-    else dr with dr_xfer := dr.dr_xfer with state := dr_xfer_read_txs
-  | dr_xfer_write_dataO => dr
-  | dr_xfer_read_rxs => dr
-  | dr_xfer_check_rxs => if rxs = 1w
-    then dr with dr_xfer := dr.dr_xfer with state := dr_xfer_read_rx0
-    else dr with dr_xfer := dr.dr_xfer with state := dr_xfer_read_rxs
-  | dr_xfer_read_rx0 => dr
-  | dr_xfer_fetch_dataI => dr
-  | dr_xfer_issue_disable => dr
-  | dr_xfer_reset_conf => dr`
-
-(* dr_check_ch0stat:driver_state -> word32 -> driver_state *)
-val dr_check_ch0stat_def = Define `
-dr_check_ch0stat (dr:driver_state) (rep_v:word32) =
-if (dr.dr_init.state = dr_init_done) /\ (dr.dr_tx.state <> dr_tx_idle) /\
-   (dr.dr_rx.state = dr_rx_idle) /\ (dr.dr_xfer.state = dr_xfer_idle)
-then (dr_check_tx_ch0stat dr rep_v)
-else if (dr.dr_init.state = dr_init_done) /\ (dr.dr_tx.state = dr_tx_idle) /\
-   (dr.dr_rx.state <> dr_rx_idle) /\ (dr.dr_xfer.state = dr_xfer_idle)
-then (dr_check_rx_ch0stat dr rep_v)
-else if (dr.dr_init.state = dr_init_done) /\ (dr.dr_tx.state = dr_tx_idle) /\
-   (dr.dr_rx.state = dr_rx_idle) /\ (dr.dr_xfer.state <> dr_xfer_idle)
-then (dr_check_xfer_ch0stat dr rep_v)
-(* other states cannot process this reply *)
-else dr`
+if (dr.state = dr_xfer_check_txs) /\ (txs = 1w) then 
+dr with state := dr_xfer_write_dataO
+else if (dr.state = dr_xfer_check_txs) /\ (txs = 0w) then
+dr with state := dr_xfer_read_txs
+else if (dr.state = dr_xfer_check_rxs) /\ (rxs = 1w) then
+dr with state := dr_xfer_read_rx0
+else if (dr.state = dr_xfer_check_rxs) /\ (rxs = 0w) then
+dr with state := dr_xfer_read_rxs
+else dr with dr_err := T`
 
 (* dr_check_rx0:driver_state -> word32 -> driver_state *)
 val dr_check_rx0_def = Define `
 dr_check_rx0 (dr:driver_state) (rep_v:word32) =
 let v = (7 >< 0) rep_v:word8 in
-if (dr.dr_rx.state = dr_rx_fetch_data) /\ (dr.dr_rx.rx_left_length > 1)
-then dr with dr_rx := dr.dr_rx with 
-     <|state := dr_rx_read_rxs; rx_data_buf := dr.dr_rx.rx_data_buf ++ [v];
-       rx_left_length := dr.dr_rx.rx_left_length - 1|>
-else if (dr.dr_rx.state = dr_rx_fetch_data) /\ (dr.dr_rx.rx_left_length = 1)
-then dr with dr_rx := dr.dr_rx with state := dr_rx_issue_disable
-else if (dr.dr_xfer.state = dr_xfer_fetch_dataI)
-then dr with dr_xfer := dr.dr_xfer with
-     <|state := if (dr.dr_xfer.xfer_cur_length < (LENGTH dr.dr_xfer.xfer_dataOUT_buf)) 
-                then dr_xfer_read_txs else dr_xfer_issue_disable; 
-       xfer_dataIN_buf := dr.dr_xfer.xfer_dataIN_buf ++ [v]|>
-else dr`
+if (dr.state = dr_rx_fetch_data) then
+dr with <| dr_rx := dr.dr_rx with <| rx_data_buf := dr.dr_rx.rx_data_buf ++ [v];
+rx_left_length := dr.dr_rx.rx_left_length - 1 |>;
+state := if dr.dr_rx.rx_left_length > 1 then dr_rx_read_rxs else dr_rx_issue_disable |>
+else if (dr.state = dr_xfer_fetch_dataI) then
+dr with <| dr_xfer := dr.dr_xfer with xfer_dataIN_buf := dr.dr_xfer.xfer_dataIN_buf ++ [v];
+state := if (dr.dr_xfer.xfer_cur_length < (LENGTH dr.dr_xfer.xfer_dataOUT_buf)) 
+then dr_xfer_read_txs else dr_xfer_issue_disable |>
+else dr with dr_err := T`
 
-(* dr_check:driver_state -> word32 -> word32 -> driver_state *)
+(* dr_check: driver_state -> word32 -> word32 -> driver_state *)
 val dr_check_def = Define `
-dr_check (dr:driver_state) (rep_ad:word32) (rep_v:word32) =
-(* driver is in an error state *)
-if dr.dr_err then dr
-(* only SYSSTATUS, CHOSTAT, RX0 should be handled *)
-else if rep_ad = SPI0_SYSSTATUS then (dr_check_sysstatus dr rep_v)
-else if rep_ad = SPI0_CH0STAT then (dr_check_ch0stat dr rep_v)
-else if rep_ad = SPI0_RX0 then (dr_check_rx0 dr rep_v)
-(* address not handled *)
-else dr`
+dr_check (dr:driver_state) (ad:word32) (v:word32) =
+case dr.state of
+  | dr_init_pre => dr with dr_err := T
+  | dr_init_idle => dr with dr_err := T
+  | dr_init_read_req => dr with dr_err := T
+  | dr_init_check_rep => if (ad = SPI0_SYSSTATUS) then (dr_check_sysstatus dr v)
+    else dr with dr_err := T
+  | dr_init_setting => dr with dr_err := T
+  | dr_ready => dr with dr_err := T
+  | dr_tx_idle => dr with dr_err := T
+  | dr_tx_conf_issued => dr with dr_err := T
+  | dr_tx_read_txs => dr with dr_err := T
+  | dr_tx_check_txs => if (ad = SPI0_CH0STAT) then (dr_check_tx_ch0stat dr v)
+    else dr with dr_err := T
+  | dr_tx_write_data => dr with dr_err := T
+  | dr_tx_read_eot => dr with dr_err := T 
+  | dr_tx_check_eot => if (ad = SPI0_CH0STAT) then (dr_check_tx_ch0stat dr v)
+    else dr with dr_err := T
+  | dr_tx_issue_disable => dr with dr_err := T
+  | dr_tx_reset_conf => dr with dr_err := T
+  | dr_rx_idle => dr with dr_err := T
+  | dr_rx_conf_issued => dr with dr_err := T
+  | dr_rx_read_rxs => dr with dr_err := T
+  | dr_rx_check_rxs => if (ad = SPI0_CH0STAT) then (dr_check_rx_ch0stat dr v)
+    else dr with dr_err := T
+  | dr_rx_read_rx0 => dr with dr_err := T
+  | dr_rx_fetch_data => if (ad = SPI0_RX0) then (dr_check_rx0 dr v)
+    else dr with dr_err := T
+  | dr_rx_issue_disable => dr with dr_err := T
+  | dr_rx_reset_conf => dr with dr_err := T
+  | dr_xfer_idle => dr with dr_err := T
+  | dr_xfer_conf_issued => dr with dr_err := T
+  | dr_xfer_read_txs => dr with dr_err := T
+  | dr_xfer_check_txs => if (ad = SPI0_CH0STAT) then (dr_check_xfer_ch0stat dr v)
+    else dr with dr_err := T
+  | dr_xfer_write_dataO => dr with dr_err := T
+  | dr_xfer_read_rxs => dr with dr_err := T
+  | dr_xfer_check_rxs => if (ad = SPI0_CH0STAT) then (dr_check_xfer_ch0stat dr v)
+    else dr with dr_err := T
+  | dr_xfer_read_rx0 => dr with dr_err := T
+  | dr_xfer_fetch_dataI => if (ad = SPI0_RX0) then (dr_check_rx0 dr v)
+    else dr with dr_err := T
+  | dr_xfer_issue_disable => dr with dr_err := T
+  | dr_xfet_reset_conf => dr with dr_err := T`
 
 val _ = export_theory();
