ds_abs1/ds_abs1_rxScript.sml
@@ -1,233 +1,171 @@
 open HolKernel bossLib boolLib Parse;
 open listTheory;
 open ds_abs1_stateTheory;
-open board_memTheory;
 
 val _ = new_theory "ds_abs1_rx";
 
 (* SPI_ABS1_RX_ENABLE: ds_abs1_state -> bool *)
 val SPI_ABS1_RX_ENABLE_def = Define `
 SPI_ABS1_RX_ENABLE (ds_abs1:ds_abs1_state) =
-((ds_abs1.ds_abs1_rx.state = abs1_rx_idle) \/
-(ds_abs1.ds_abs1_rx.state = abs1_rx_update) \/
-(ds_abs1.ds_abs1_rx.state = abs1_rx_fetch_data) \/
-(ds_abs1.ds_abs1_rx.state = abs1_rx_return) \/
-(ds_abs1.ds_abs1_rx.state = abs1_rx_check_1) \/
-(ds_abs1.ds_abs1_rx.state = abs1_rx_pre_reset) \/
-(ds_abs1.ds_abs1_rx.state = abs1_rx_ready_for_reset))`
+((ds_abs1.state = abs1_rx_idle) \/
+(ds_abs1.state = abs1_rx_update) \/
+(ds_abs1.state = abs1_rx_next) \/
+(ds_abs1.state = abs1_rx_stop))`
 
 (* DRIVER_ABS1_RX_ENABLE: ds_abs1_state -> bool *)
 val DRIVER_ABS1_RX_ENABLE_def = Define `
 DRIVER_ABS1_RX_ENABLE (ds_abs1:ds_abs1_state) =
-((ds_abs1.ds_abs1_rx.state = abs1_rx_ready) \/
-(ds_abs1.ds_abs1_rx.state = abs1_rx_fetch_data) \/
-(ds_abs1.ds_abs1_rx.state = abs1_rx_done) \/
-(ds_abs1.ds_abs1_rx.state = abs1_rx_check_1) \/
-(ds_abs1.ds_abs1_rx.state = abs1_rx_check_2))`
+((ds_abs1.state = abs1_rx_ready) \/
+(ds_abs1.state = abs1_rx_fetch_data) \/
+(ds_abs1.state = abs1_rx_next) \/
+(ds_abs1.state = abs1_rx_next_ready))`
 
 (* COMB_ABS1_RX_ENABLE: ds_abs1_state -> bool *)
 val COMB_ABS1_RX_ENABLE_def = Define `
 COMB_ABS1_RX_ENABLE (ds_abs1:ds_abs1_state) =
-((ds_abs1.ds_abs1_rx.state = abs1_rx_reset) \/
-(ds_abs1.ds_abs1_rx.state = abs1_rx_ready_for_reset))`
+(ds_abs1.state = abs1_rx_reset)`
 
 (* ABS1_RX_LBL_ENABLE: ds_abs1_state -> bool *)
 val ABS1_RX_LBL_ENABLE_def = Define `
 ABS1_RX_LBL_ENABLE (ds_abs1:ds_abs1_state) =
-((ds_abs1.ds_abs1_rx.state = abs1_rx_receive) \/
-(ds_abs1.ds_abs1_rx.state = abs1_rx_done) \/
-(ds_abs1.ds_abs1_rx.state = abs1_rx_last))`
+((ds_abs1.state = abs1_rx_receive) \/
+(ds_abs1.state = abs1_rx_fetch_data) \/
+(ds_abs1.state = abs1_rx_done))`
 
 (* tau_spi related functions *)
 (* spi_abs1_rx_idle_op: ds_abs1_state -> ds_abs1_state *)
 val spi_abs1_rx_idle_op_def = Define `
 spi_abs1_rx_idle_op (ds_abs1:ds_abs1_state) =
-ds_abs1 with
-ds_abs1_rx := ds_abs1.ds_abs1_rx with
-state := abs1_rx_receive`
+ds_abs1 with state := abs1_rx_receive`
 
 (* spi_abs1_rx_update_op: ds_abs1_state -> ds_abs1_state *)
 val spi_abs1_rx_update_op_def = Define `
 spi_abs1_rx_update_op (ds_abs1:ds_abs1_state) =
-ds_abs1 with ds_abs1_rx := ds_abs1.ds_abs1_rx with
-state := abs1_rx_ready`
+ds_abs1 with state := abs1_rx_ready`
 
-(* spi_abs1_rx_fetch_data_op: ds_abs1_state -> ds_abs1_state *)
-val spi_abs1_rx_fetch_data_op_def = Define `
-spi_abs1_rx_fetch_data_op (ds_abs1:ds_abs1_state) =
-ds_abs1 with ds_abs1_rx := ds_abs1.ds_abs1_rx with
-state := abs1_rx_done`
+(* spi_abs1_rx_next_op: ds_abs1_state -> ds_abs1_state *)
+val spi_abs1_rx_next_op_def = Define `
+spi_abs1_rx_next_op (ds_abs1:ds_abs1_state) =
+ds_abs1 with state := abs1_rx_next_ready`
 
-(* spi_abs1_rx_return_op: ds_abs1_state -> ds_abs1_state *)
-val spi_abs1_rx_return_op_def = Define `
-spi_abs1_rx_return_op (ds_abs1:ds_abs1_state) =
-ds_abs1 with ds_abs1_rx := ds_abs1.ds_abs1_rx with
-state := abs1_rx_receive`
-
-(* spi_abs1_rx_check_1_op: ds_abs1_state -> ds_abs1_state *)
-val spi_abs1_rx_check_1_op_def = Define `
-spi_abs1_rx_check_1_op (ds_abs1:ds_abs1_state) =
-ds_abs1 with ds_abs1_rx := ds_abs1.ds_abs1_rx with
-state := abs1_rx_check_2`
-
-(* spi_abs1_rx_pre_reset_op: ds_abs1_state -> ds_abs1_state *)
-val spi_abs1_rx_pre_reset_op_def = Define `
-spi_abs1_rx_pre_reset_op (ds_abs1:ds_abs1_state) =
-ds_abs1 with ds_abs1_rx := ds_abs1.ds_abs1_rx with
-state := abs1_rx_reset`
-
-(* spi_abs1_rx_ready_for_reset_op: ds_abs1_state -> ds_abs1_state *)
-val spi_abs1_rx_ready_for_reset_op_def = Define `
-spi_abs1_rx_ready_for_reset_op (ds_abs1:ds_abs1_state) =
-ds_abs1 with ds_abs1_rx := ds_abs1.ds_abs1_rx with
-state := abs1_rx_last`
+(* spi_abs1_rx_stop_op: ds_abs1_state -> ds_abs1_state *)
+val spi_abs1_rx_stop_op_def = Define `
+spi_abs1_rx_stop_op (ds_abs1:ds_abs1_state) =
+ds_abs1 with state := abs1_rx_reset`
 
 (* spi_abs_rx_operations: ds_abs1_state -> ds_abs1_state *)
 val spi_abs1_rx_operations_def = Define `
 spi_abs1_rx_operations (ds_abs1:ds_abs1_state) =
-case ds_abs1.ds_abs1_rx.state of
-  | abs1_rx_pre => ds_abs1 with err := T
-  | abs1_rx_idle => spi_abs1_rx_idle_op ds_abs1
-  | abs1_rx_receive => ds_abs1 with err := T
-  | abs1_rx_update => spi_abs1_rx_update_op ds_abs1
-  | abs1_rx_ready => ds_abs1 with err := T
-  | abs1_rx_fetch_data => spi_abs1_rx_fetch_data_op ds_abs1
-  | abs1_rx_return => spi_abs1_rx_return_op ds_abs1
-  | abs1_rx_done => ds_abs1 with err := T
-  | abs1_rx_last => ds_abs1 with err := T
-  | abs1_rx_check_1 => spi_abs1_rx_check_1_op ds_abs1
-  | abs1_rx_check_2 => ds_abs1 with err := T
-  | abs1_rx_pre_reset => spi_abs1_rx_pre_reset_op ds_abs1
-  | abs1_rx_ready_for_reset => spi_abs1_rx_ready_for_reset_op ds_abs1
-  | abs1_rx_reset => ds_abs1 with err := T`
+if (ds_abs1.state = abs1_rx_idle) then
+(spi_abs1_rx_idle_op ds_abs1)
+else if (ds_abs1.state = abs1_rx_update) then
+(spi_abs1_rx_update_op ds_abs1)
+else if (ds_abs1.state = abs1_rx_next) then
+(spi_abs1_rx_next_op ds_abs1)
+else if (ds_abs1.state = abs1_rx_stop) then
+(spi_abs1_rx_stop_op ds_abs1)
+else ds_abs1 with err := T`
 
 
 (* tau_dr related functions *)
 (* driver_abs1_rx_ready_op: ds_abs1_state -> ds_abs1_state *)
 val driver_abs1_rx_ready_op_def = Define `
 driver_abs1_rx_ready_op (ds_abs1:ds_abs1_state) =
-ds_abs1 with ds_abs1_rx := ds_abs1.ds_abs1_rx with 
-state := abs1_rx_fetch_data`
+ds_abs1 with state := abs1_rx_fetch_data`
 
 (* driver_abs1_rx_fetch_data_op: ds_abs1_state -> ds_abs1_state *)
 val driver_abs1_rx_fetch_data_op_def = Define `
 driver_abs1_rx_fetch_data_op (ds_abs1:ds_abs1_state) =
-ds_abs1 with ds_abs1_rx := ds_abs1.ds_abs1_rx with
-<| state := if ds_abs1.ds_abs1_rx.rx_left_length > 1 then abs1_rx_return
-   else abs1_rx_ready_for_reset;
-   rx_data_buffer := ds_abs1.ds_abs1_rx.rx_data_buffer ++ [ds_abs1.spi_abs1.RX_SHIFT_REG]; 
-   rx_left_length := ds_abs1.ds_abs1_rx.rx_left_length - 1 |>`
+ds_abs1 with <| ds_abs1_rx := ds_abs1.ds_abs1_rx with
+<| rx_data_buffer := ds_abs1.ds_abs1_rx.rx_data_buffer ++ [ds_abs1.spi_abs1.RX_SHIFT_REG]; 
+   rx_left_length := ds_abs1.ds_abs1_rx.rx_left_length - 1 |>;
+state := if ds_abs1.ds_abs1_rx.rx_left_length > 1 then abs1_rx_done else abs1_rx_receive |>`
 
-(* driver_abs1_rx_done_op: ds_abs1_state -> ds_abs1_state *)
-val driver_abs1_rx_done_op_def = Define `
-driver_abs1_rx_done_op (ds_abs1:ds_abs1_state) =
-ds_abs1 with ds_abs1_rx := ds_abs1.ds_abs1_rx with
-<| state := if ds_abs1.ds_abs1_rx.rx_left_length > 1 then abs1_rx_receive
-   else abs1_rx_reset;
-   rx_data_buffer := ds_abs1.ds_abs1_rx.rx_data_buffer ++ [ds_abs1.spi_abs1.RX_SHIFT_REG];
-   rx_left_length := ds_abs1.ds_abs1_rx.rx_left_length - 1 |>`
+(* driver_abs1_rx_next_op: ds_abs1_state -> ds_abs1_state *)
+val driver_abs1_rx_next_op_def = Define `
+driver_abs1_rx_next_op (ds_abs1:ds_abs1_state) =
+ds_abs1 with <| ds_abs1_rx := ds_abs1.ds_abs1_rx with
+<| rx_data_buffer := ds_abs1.ds_abs1_rx.rx_data_buffer ++ [ds_abs1.ds_abs1_rx.temp_value];
+   rx_left_length := ds_abs1.ds_abs1_rx.rx_left_length - 1 |>;
+state := if ds_abs1.ds_abs1_rx.rx_left_length > 1 then abs1_rx_update else abs1_rx_stop |>`
 
-(* driver_abs1_rx_check_1_op: ds_abs1_state -> ds_abs1_state *)
-val driver_abs1_rx_check_1_op_def = Define `
-driver_abs1_rx_check_1_op (ds_abs1: ds_abs1_state) =
-ds_abs1 with ds_abs1_rx := ds_abs1.ds_abs1_rx with 
-<| state := if ds_abs1.ds_abs1_rx.rx_left_length > 1 then abs1_rx_update
-   else abs1_rx_pre_reset;
-   rx_data_buffer := ds_abs1.ds_abs1_rx.rx_data_buffer ++ [ds_abs1.spi_abs1.RX_SHIFT_REG];
-   rx_left_length := ds_abs1.ds_abs1_rx.rx_left_length - 1 |>`
-
-(* driver_abs1_rx_check_2_op: ds_abs1_state -> ds_abs1_state *)
-val driver_abs1_rx_check_2_op_def = Define `
-driver_abs1_rx_check_2_op (ds_abs1: ds_abs1_state) =
-ds_abs1 with ds_abs1_rx := ds_abs1.ds_abs1_rx with
-<| state := if ds_abs1.ds_abs1_rx.rx_left_length > 1 then abs1_rx_ready
-   else abs1_rx_reset;
-   rx_data_buffer := ds_abs1.ds_abs1_rx.rx_data_buffer ++ [ds_abs1.spi_abs1.RX_SHIFT_REG];
-   rx_left_length := ds_abs1.ds_abs1_rx.rx_left_length - 1 |>`
+(* driver_abs1_rx_next_ready_op: ds_abs1_state -> ds_abs1_state *)
+val driver_abs1_rx_next_ready_op_def = Define `
+driver_abs1_rx_next_ready_op (ds_abs1: ds_abs1_state) =
+ds_abs1 with <| ds_abs1_rx := ds_abs1.ds_abs1_rx with 
+<| rx_data_buffer := ds_abs1.ds_abs1_rx.rx_data_buffer ++ [ds_abs1.ds_abs1_rx.temp_value];
+   rx_left_length := ds_abs1.ds_abs1_rx.rx_left_length - 1 |>;
+state := if ds_abs1.ds_abs1_rx.rx_left_length > 1 then abs1_rx_ready else abs1_rx_reset |>`
 
 (* driver_abs1_rx_operations: ds_abs1_state -> ds_abs1_state *)
 val driver_abs1_rx_operations_def = Define `
 driver_abs1_rx_operations (ds_abs1:ds_abs1_state) =
-case ds_abs1.ds_abs1_rx.state of
-  | abs1_rx_pre => ds_abs1 with err := T
-  | abs1_rx_idle => ds_abs1 with err := T
-  | abs1_rx_receive => ds_abs1 with err := T
-  | abs1_rx_update => ds_abs1 with err := T
-  | abs1_rx_ready => driver_abs1_rx_ready_op ds_abs1
-  | abs1_rx_fetch_data => driver_abs1_rx_fetch_data_op ds_abs1
-  | abs1_rx_return => ds_abs1 with err := T
-  | abs1_rx_done => driver_abs1_rx_done_op ds_abs1
-  | abs1_rx_last => ds_abs1 with err := T
-  | abs1_rx_check_1 => driver_abs1_rx_check_1_op ds_abs1
-  | abs1_rx_check_2 => driver_abs1_rx_check_2_op ds_abs1
-  | abs1_rx_pre_reset => ds_abs1 with err := T
-  | abs1_rx_ready_for_reset => ds_abs1 with err := T
-  | abs1_rx_reset => ds_abs1 with err := T`
+if (ds_abs1.state = abs1_rx_ready) then
+(driver_abs1_rx_ready_op ds_abs1)
+else if (ds_abs1.state = abs1_rx_fetch_data) then
+(driver_abs1_rx_fetch_data_op ds_abs1)
+else if (ds_abs1.state = abs1_rx_next) then
+(driver_abs1_rx_next_op ds_abs1)
+else if (ds_abs1.state = abs1_rx_next_ready) then
+(driver_abs1_rx_next_ready_op ds_abs1)
+else ds_abs1 with err:= T`
 
 
 (* tau_comb related functions *)
-(* comb_abs1_rx_ready_for_reset_op: ds_abs1_state -> ds_abs1_state *)
-val comb_abs1_rx_ready_for_reset_op_def = Define `
-comb_abs1_rx_ready_for_reset_op (ds_abs1:ds_abs1_state) =
-ds_abs1 with ds_abs1_rx := ds_abs1.ds_abs1_rx with state := abs1_rx_reset`
-
 (* comb_abs1_rx_reset_op: ds_abs1_state -> ds_abs1_state *)
 val comb_abs1_rx_reset_op_def = Define `
 comb_abs1_rx_reset_op (ds_abs1:ds_abs1_state) =
-ds_abs1 with ds_abs1_rx := ds_abs1.ds_abs1_rx with state := abs1_rx_pre`
+ds_abs1 with state := abs1_ready`
 
 (* comb_abs1_rx_operations: ds_abs1_state -> ds_abs1_state *)
 val comb_abs1_rx_operations_def = Define `
 comb_abs1_rx_operations (ds_abs1:ds_abs1_state) =
-if ds_abs1.ds_abs1_rx.state = abs1_rx_ready_for_reset
-then (comb_abs1_rx_ready_for_reset_op ds_abs1)
-else if ds_abs1.ds_abs1_rx.state = abs1_rx_reset
+if ds_abs1.state = abs1_rx_reset
 then (comb_abs1_rx_reset_op ds_abs1)
 else ds_abs1 with err := T`
+
 
 (* call_rx_ds_abs1: ds_abs1_state -> num -> ds_abs1_state *)
 val call_rx_ds_abs1_def = Define `
 call_rx_ds_abs1 (ds_abs1:ds_abs1_state) (length: num) =
-ds_abs1 with ds_abs1_rx := ds_abs1.ds_abs1_rx with
-<| state := abs1_rx_idle;
-rx_left_length := length;
-rx_data_buffer := [] |>`
+ds_abs1 with <| ds_abs1_rx := ds_abs1.ds_abs1_rx with
+<| rx_left_length := length; rx_data_buffer := [] |>;
+state := abs1_rx_idle |>`
+
 
 (* RX label function *)
 (* abs1_rx_receive_op: ds_abs1_state -> word8 option -> ds_abs1_state *)
 val abs1_rx_receive_op_def = Define `
 abs1_rx_receive_op (ds_abs1:ds_abs1_state) (data: word8 option) =
-if (data <> NONE) then
 ds_abs1 with 
-<| ds_abs1_rx := ds_abs1.ds_abs1_rx with state := abs1_rx_update;
-   spi_abs1 := ds_abs1.spi_abs1 with RX_SHIFT_REG := THE data |>
-else ds_abs1`
+<| state := abs1_rx_update;
+   spi_abs1 := ds_abs1.spi_abs1 with RX_SHIFT_REG := THE data |>`
+
+(* abs1_rx_fetch_data_op: ds_abs1_state -> word8 option -> ds_abs1_state *)
+val abs1_rx_fetch_data_op_def = Define `
+abs1_rx_fetch_data_op (ds_abs1:ds_abs1_state) (data:word8 option) =
+ds_abs1 with 
+<| state := abs1_rx_next;
+   spi_abs1 := ds_abs1.spi_abs1 with RX_SHIFT_REG := THE data;
+   ds_abs1_rx := ds_abs1.ds_abs1_rx with temp_value := ds_abs1.spi_abs1.RX_SHIFT_REG |>`
 
 (* abs1_rx_done_op: ds_abs1_state -> word8 option -> ds_abs1_state *)
 val abs1_rx_done_op_def = Define `
 abs1_rx_done_op (ds_abs1:ds_abs1_state) (data:word8 option) =
-if (data <> NONE) then
 ds_abs1 with 
-<| ds_abs1_rx := ds_abs1.ds_abs1_rx with state := abs1_rx_check_1;
-   spi_abs1 := ds_abs1.spi_abs1 with RX_SHIFT_REG := THE data |>
-else ds_abs1`
-
-(* abs1_rx_last_op: ds_abs1_state -> word8 option -> ds_abs1_state *)
-val abs1_rx_last_op_def = Define `
-abs1_rx_last_op (ds_abs1:ds_abs1_state) (data:word8 option) =
-if (data <> NONE) then
-ds_abs1 with 
-<| ds_abs1_rx := ds_abs1.ds_abs1_rx with state := abs1_rx_pre_reset;
-   spi_abs1 := ds_abs1.spi_abs1 with RX_SHIFT_REG := THE data |>
-else ds_abs1`
+<| state := abs1_rx_stop;
+   spi_abs1 := ds_abs1.spi_abs1 with RX_SHIFT_REG := THE data |>`
 
 
 (* abs1_rx_receive_data_op: ds_abs1_state -> word8 option -> ds_abs1_state *)
 val abs1_rx_receive_data_op_def = Define `
 abs1_rx_receive_data_op (ds_abs1:ds_abs1_state) (data:word8 option) =
-if ds_abs1.ds_abs1_rx.state = abs1_rx_receive then (abs1_rx_receive_op ds_abs1 data)
-else if ds_abs1.ds_abs1_rx.state = abs1_rx_done then (abs1_rx_done_op ds_abs1 data)
-else if ds_abs1.ds_abs1_rx.state = abs1_rx_last then (abs1_rx_last_op ds_abs1 data)
+if (ds_abs1.state = abs1_rx_receive) then 
+(abs1_rx_receive_op ds_abs1 data)
+else if (ds_abs1.state = abs1_rx_fetch_data) then 
+(abs1_rx_fetch_data_op ds_abs1 data)
+else if (ds_abs1.state = abs1_rx_done) then 
+(abs1_rx_done_op ds_abs1 data)
 else ds_abs1 with err := T`
 
 val _ = export_theory();
