ds_abs1/ds_abs1_txScript.sml
@@ -1,48 +1,32 @@
 open HolKernel bossLib boolLib Parse;
 open listTheory;
 open ds_abs1_stateTheory;
-open board_memTheory;
 
 val _ = new_theory "ds_abs1_tx";
 
 (* SPI_ABS1_TX_ENABLE: ds_abs1_state -> bool *)
 val SPI_ABS1_TX_ENABLE_def = Define `
 SPI_ABS1_TX_ENABLE (ds_abs1:ds_abs1_state) =
-((ds_abs1.ds_abs1_tx.state = abs1_tx_idle) \/ 
-(ds_abs1.ds_abs1_tx.state = abs1_tx_data_1) \/
-(ds_abs1.ds_abs1_tx.state = abs1_tx_data_2) \/
-(ds_abs1.ds_abs1_tx.state = abs1_tx_check_1) \/ 
-(ds_abs1.ds_abs1_tx.state = abs1_tx_check_3) \/
-(ds_abs1.ds_abs1_tx.state = abs1_tx_next) \/ 
-(ds_abs1.ds_abs1_tx.state = abs1_tx_ready_for_reset))`
-
-(* DRIVER_ABS1_TX_ENABLE: ds_abs1_state -> bool *)
-val DRIVER_ABS1_TX_ENABLE_def = Define `
-DRIVER_ABS1_TX_ENABLE (ds_abs1:ds_abs1_state) =
-((ds_abs1.ds_abs1_tx.state = abs1_tx_prepare) \/
-(ds_abs1.ds_abs1_tx.state = abs1_tx_done_2) \/
-(ds_abs1.ds_abs1_tx.state = abs1_tx_check_1) \/
-(ds_abs1.ds_abs1_tx.state = abs1_tx_check_2) \/
-(ds_abs1.ds_abs1_tx.state = abs1_tx_check_3))`
+((ds_abs1.state = abs1_tx_idle) \/ 
+(ds_abs1.state = abs1_tx_data_1) \/
+(ds_abs1.state = abs1_tx_data_2))`
 
 (* COMB_ABS1_TX_ENABLE: ds_abs1_state -> bool *)
 val COMB_ABS1_TX_ENABLE_def = Define `
 COMB_ABS1_TX_ENABLE (ds_abs1:ds_abs1_state) =
-((ds_abs1.ds_abs1_tx.state = abs1_tx_trans) \/
-(ds_abs1.ds_abs1_tx.state = abs1_tx_reset) \/
-(ds_abs1.ds_abs1_tx.state = abs1_tx_ready_for_reset))`
+((ds_abs1.state = abs1_tx_trans) \/
+(ds_abs1.state = abs1_tx_reset))`
 
 (* tau_spi related functions *)
 (* spi_abs1_tx_idle_op: ds_abs1_state -> ds_abs1_state *)
 val spi_abs1_tx_idle_op_def = Define `
 spi_abs1_tx_idle_op (ds_abs1:ds_abs1_state) =
-ds_abs1 with ds_abs1_tx := ds_abs1.ds_abs1_tx with 
-state := abs1_tx_prepare`
+ds_abs1 with state := abs1_tx_trans`
 
 (* spi_abs1_tx_data_1_op: ds_abs1_state -> ds_abs1_state *)
 val spi_abs1_tx_data_1_op_def = Define `
 spi_abs1_tx_data_1_op (ds_abs1:ds_abs1_state) =
-ds_abs1 with <| ds_abs1_tx := ds_abs1.ds_abs1_tx with state := abs1_tx_done_1;
+ds_abs1 with <| state := abs1_tx_done_1;
 spi_abs1 := ds_abs1.spi_abs1 with
 TX_SHIFT_REG := (EL (ds_abs1.ds_abs1_tx.tx_cur_length - 1) 
 (ds_abs1.ds_abs1_tx.tx_data_buffer)) |>`
@@ -50,139 +34,43 @@ TX_SHIFT_REG := (EL (ds_abs1.ds_abs1_tx.tx_cur_length - 1)
 (* spi_abs1_tx_data_2_op: ds_abs1_state -> ds_abs1_state *)
 val spi_abs1_tx_data_2_op_def = Define `
 spi_abs1_tx_data_2_op (ds_abs1:ds_abs1_state) =
-ds_abs1 with <| ds_abs1_tx := ds_abs1.ds_abs1_tx with state := abs1_tx_done_2;
+ds_abs1 with <| state := abs1_tx_done_2;
 spi_abs1 := ds_abs1.spi_abs1 with
 TX_SHIFT_REG := (EL (ds_abs1.ds_abs1_tx.tx_cur_length - 1) 
 (ds_abs1.ds_abs1_tx.tx_data_buffer)) |>`
 
-(* spi_abs1_check_1_op: ds_abs1_state -> ds_abs1_state *)
-val spi_abs1_tx_check_1_op_def = Define `
-spi_abs1_tx_check_1_op (ds_abs1:ds_abs1_state) = 
-ds_abs1 with ds_abs1_tx := ds_abs1.ds_abs1_tx with
-state := abs1_tx_check_2`
-
-(* spi_abs1_check_3_op: ds_abs1_state -> ds_abs1_state *)
-val spi_abs1_tx_check_3_op_def = Define `
-spi_abs1_tx_check_3_op (ds_abs1:ds_abs1_state) =
-ds_abs1 with ds_abs1_tx := ds_abs1.ds_abs1_tx with
-state := abs1_tx_prepare`
-
-(* spi_abs1_tx_next_op: ds_abs1_state -> ds_abs1_state *)
-val spi_abs1_tx_next_op_def = Define `
-spi_abs1_tx_next_op (ds_abs1:ds_abs1_state) =
-ds_abs1 with ds_abs1_tx := ds_abs1.ds_abs1_tx with
-state := abs1_tx_trans`
-
-(* spi_abs1_tx_ready_for_reset_op: ds_abs1_state -> ds_abs1_state *)
-val spi_abs1_tx_ready_for_reset_op_def = Define `
-spi_abs1_tx_ready_for_reset_op (ds_abs1:ds_abs1_state) =
-ds_abs1 with ds_abs1_tx := ds_abs1.ds_abs1_tx with
-state := abs1_tx_reset`
-
 (* spi_abs1_tx_operations: ds_abs1_state -> ds_abs1_state *)
 val spi_abs1_tx_operations_def = Define `
 spi_abs1_tx_operations (ds_abs1:ds_abs1_state) =
-case ds_abs1.ds_abs1_tx.state of
-  | abs1_tx_not_ready => ds_abs1 with err := T
-  | abs1_tx_pre => ds_abs1 with err := T
-  | abs1_tx_idle => spi_abs1_tx_idle_op ds_abs1
-  | abs1_tx_prepare => ds_abs1 with err := T
-  | abs1_tx_trans => ds_abs1 with err := T
-  | abs1_tx_data_1 => spi_abs1_tx_data_1_op ds_abs1
-  | abs1_tx_data_2 => spi_abs1_tx_data_2_op ds_abs1
-  | abs1_tx_done_1 => ds_abs1 with err := T
-  | abs1_tx_done_2 => ds_abs1 with err := T
-  | abs1_tx_done_3 => ds_abs1 with err := T
-  | abs1_tx_check_1 => spi_abs1_tx_check_1_op ds_abs1
-  | abs1_tx_check_2 => ds_abs1 with err := T
-  | abs1_tx_check_3 => spi_abs1_tx_check_3_op ds_abs1
-  | abs1_tx_next => spi_abs1_tx_next_op ds_abs1
-  | abs1_tx_ready_for_reset => spi_abs1_tx_ready_for_reset_op ds_abs1 
-  | abs1_tx_reset => ds_abs1 with err := T`
-
-
-(* tau_dr related functions *)
-
-(* driver_abs1_tx_prepare_op: ds_abs1_state -> ds_abs1_state *)
-val driver_abs1_tx_prepare_op_def = Define `
-driver_abs1_tx_prepare_op (ds_abs1:ds_abs1_state) =
-ds_abs1 with ds_abs1_tx := ds_abs1.ds_abs1_tx with 
-state := abs1_tx_trans`
-
-(* driver_abs1_tx_done_2_op: ds_abs1_state -> ds_abs1_state *)
-val driver_abs1_tx_done_2_op_def = Define `
-driver_abs1_tx_done_2_op (ds_abs1:ds_abs1_state) =
-ds_abs1 with ds_abs1_tx := ds_abs1.ds_abs1_tx with 
-state := abs1_tx_done_3`
-
-(* driver_abs1_tx_check_1_op: ds_abs1_state -> ds_abs1_state *)
-val driver_abs1_tx_check_1_op_def = Define `
-driver_abs1_tx_check_1_op (ds_abs1:ds_abs1_state) =
-ds_abs1 with ds_abs1_tx := ds_abs1.ds_abs1_tx with 
-state := abs1_tx_ready_for_reset`
-
-(* driver_abs1_tx_check_2_op: ds_abs1_state -> ds_abs1_state *)
-val driver_abs1_tx_check_2_op_def = Define `
-driver_abs1_tx_check_2_op (ds_abs1:ds_abs1_state) =
-ds_abs1 with ds_abs1_tx := ds_abs1.ds_abs1_tx with 
-state := abs1_tx_reset`
-
-(* driver_abs1_tx_check_3_op: ds_abs1_state -> ds_abs1_state *)
-val driver_abs1_tx_check_3_op_def = Define `
-driver_abs1_tx_check_3_op (ds_abs1:ds_abs1_state) =
-ds_abs1 with ds_abs1_tx := ds_abs1.ds_abs1_tx with 
-state := abs1_tx_next`
-
-(* driver_abs1_tx_operations: ds_abs1_state -> ds_abs1_state *)
-val driver_abs1_tx_operations_def = Define `
-driver_abs1_tx_operations (ds_abs1:ds_abs1_state) =
-case ds_abs1.ds_abs1_tx.state of
-  | abs1_tx_not_ready => ds_abs1 with err := T
-  | abs1_tx_pre => ds_abs1 with err := T
-  | abs1_tx_idle =>  ds_abs1 with err := T
-  | abs1_tx_prepare => driver_abs1_tx_prepare_op ds_abs1
-  | abs1_tx_trans => ds_abs1 with err := T
-  | abs1_tx_data_1 => ds_abs1 with err := T
-  | abs1_tx_data_2 => ds_abs1 with err := T
-  | abs1_tx_done_1 => ds_abs1 with err := T
-  | abs1_tx_done_2 => driver_abs1_tx_done_2_op ds_abs1
-  | abs1_tx_done_3 => ds_abs1 with err := T
-  | abs1_tx_check_1 => driver_abs1_tx_check_1_op ds_abs1
-  | abs1_tx_check_2 => driver_abs1_tx_check_2_op ds_abs1
-  | abs1_tx_check_3 => driver_abs1_tx_check_3_op ds_abs1 
-  | abs1_tx_next => ds_abs1 with err := T
-  | abs1_tx_ready_for_reset => ds_abs1 with err := T
-  | abs1_tx_reset => ds_abs1 with err := T`
+if (ds_abs1.state = abs1_tx_idle) then
+(spi_abs1_tx_idle_op ds_abs1)
+else if (ds_abs1.state = abs1_tx_data_1) then
+(spi_abs1_tx_data_1_op ds_abs1)
+else if (ds_abs1.state = abs1_tx_data_2) then
+(spi_abs1_tx_data_2_op ds_abs1)
+else ds_abs1 with err := T`
 
 
 (* tau_comb related functions *)
 (* comb_abs1_tx_trans_op ds_abs1_state -> ds_abs1_state *)
 val comb_abs1_tx_trans_op_def = Define `
 comb_abs1_tx_trans_op (ds_abs1:ds_abs1_state) =
-ds_abs1 with ds_abs1_tx := ds_abs1.ds_abs1_tx with
-<| state := if ds_abs1.ds_abs1_tx.tx_cur_length < ((LENGTH ds_abs1.ds_abs1_tx.tx_data_buffer) - 1)
-   then abs1_tx_data_2 
-   else abs1_tx_data_1;
-   tx_cur_length := ds_abs1.ds_abs1_tx.tx_cur_length + 1 |>`
-
-(* comb_abs1_tx_ready_for_reset_op: ds_abs1_state -> ds_abs1_state *)
-val comb_abs1_tx_ready_for_reset_op_def = Define `
-comb_abs1_tx_ready_for_reset_op (ds_abs1:ds_abs1_state) =
-ds_abs1 with ds_abs1_tx := ds_abs1.ds_abs1_tx with state := abs1_tx_reset`
+ds_abs1 with <| 
+state := if ds_abs1.ds_abs1_tx.tx_cur_length < ((LENGTH ds_abs1.ds_abs1_tx.tx_data_buffer) - 1)
+then abs1_tx_data_2 else abs1_tx_data_1;
+ds_abs1_tx := ds_abs1.ds_abs1_tx with tx_cur_length := ds_abs1.ds_abs1_tx.tx_cur_length + 1 |>`
 
 (* comb_abs1_tx_reset_op: ds_abs1_state -> ds_abs1_state *)
 val comb_abs1_tx_reset_op_def = Define `
 comb_abs1_tx_reset_op (ds_abs1:ds_abs1_state) =
-ds_abs1 with ds_abs1_tx := ds_abs1.ds_abs1_tx with state := abs1_tx_pre`
+ds_abs1 with state := abs1_ready`
 
 (* comb_abs1_tx_operations: ds_abs1_state -> ds_abs1_state *)
 val comb_abs1_tx_operations_def = Define `
 comb_abs1_tx_operations (ds_abs1:ds_abs1_state) =
-if ds_abs1.ds_abs1_tx.state = abs1_tx_trans 
+if ds_abs1.state = abs1_tx_trans 
 then (comb_abs1_tx_trans_op ds_abs1)
-else if ds_abs1.ds_abs1_tx.state = abs1_tx_ready_for_reset
-then (comb_abs1_tx_ready_for_reset_op ds_abs1)
-else if ds_abs1.ds_abs1_tx.state = abs1_tx_reset 
+else if ds_abs1.state = abs1_tx_reset 
 then (comb_abs1_tx_reset_op ds_abs1)
 else ds_abs1 with err := T`
 
@@ -191,23 +79,19 @@ else ds_abs1 with err := T`
  *)
 val ABS1_TX_LBL_ENABLE_def = Define `
 ABS1_TX_LBL_ENABLE (ds_abs1:ds_abs1_state) =
-((ds_abs1.ds_abs1_tx.state = abs1_tx_done_1) \/
-(ds_abs1.ds_abs1_tx.state = abs1_tx_done_2) \/
-(ds_abs1.ds_abs1_tx.state = abs1_tx_done_3))`
+((ds_abs1.state = abs1_tx_done_1) \/
+(ds_abs1.state = abs1_tx_done_2))`
 
 (* abs1_tx_trans_done_op: ds_abs1_state -> ds_abs1_state * word8 option *)
 val abs1_tx_trans_done_op_def = Define `
 abs1_tx_trans_done_op (ds_abs1:ds_abs1_state) =
-if ds_abs1.ds_abs1_tx.state = abs1_tx_done_1 then
-(ds_abs1 with ds_abs1_tx := ds_abs1.ds_abs1_tx with state := abs1_tx_check_1,
+if ds_abs1.state = abs1_tx_done_1 then
+(ds_abs1 with state := abs1_tx_reset,
 SOME ds_abs1.spi_abs1.TX_SHIFT_REG)
-else if ds_abs1.ds_abs1_tx.state = abs1_tx_done_2 then
-(ds_abs1 with ds_abs1_tx := ds_abs1.ds_abs1_tx with state := abs1_tx_check_3,
+else if ds_abs1.state = abs1_tx_done_2 then
+(ds_abs1 with state := abs1_tx_trans,
 SOME ds_abs1.spi_abs1.TX_SHIFT_REG)
-else if ds_abs1.ds_abs1_tx.state = abs1_tx_done_3 then
-(ds_abs1 with ds_abs1_tx := ds_abs1.ds_abs1_tx with state := abs1_tx_next,
-SOME ds_abs1.spi_abs1.TX_SHIFT_REG)
-else (ds_abs1, NONE)`
+else (ds_abs1 with err := T, NONE)`
 
 (* abs1_tx_trans_done_op_value: ds_abs1_state -> word8 option *)
 val abs1_tx_trans_done_op_value_def = Define `
@@ -224,9 +108,8 @@ in ds_abs1'`
 (* call_tx_ds_abs1: ds_abs1_state -> word8 list -> ds_abs1_state *)
 val call_tx_ds_abs1_def = Define `
 call_tx_ds_abs1 (ds_abs1:ds_abs1_state) (buffer:word8 list) =
-ds_abs1 with ds_abs1_tx := ds_abs1.ds_abs1_tx with
-<| state := abs1_tx_idle;
-   tx_data_buffer := buffer;
-   tx_cur_length := 0 |>`
+ds_abs1 with <| ds_abs1_tx := ds_abs1.ds_abs1_tx with 
+<| tx_data_buffer := buffer; tx_cur_length := 0 |>;
+state := abs1_tx_idle |>`
 
 val _ = export_theory();
