ds_abs1/ds_abs1_xferScript.sml
@@ -1,187 +1,111 @@
 open HolKernel bossLib boolLib Parse;
 open listTheory;
 open ds_abs1_stateTheory;
-open board_memTheory;
 
 val _ = new_theory "ds_abs1_xfer";
 
 (* SPI_ABS1_XFER_ENABLE: ds_abs1_state -> bool *)
 val SPI_ABS1_XFER_ENABLE_def = Define `
 SPI_ABS1_XFER_ENABLE (ds_abs1:ds_abs1_state) =
-((ds_abs1.ds_abs1_xfer.state = abs1_xfer_idle) \/
-(ds_abs1.ds_abs1_xfer.state = abs1_xfer_data) \/
-(ds_abs1.ds_abs1_xfer.state = abs1_xfer_update) \/
-(ds_abs1.ds_abs1_xfer.state = abs1_xfer_fetch_data) \/
-(ds_abs1.ds_abs1_xfer.state = abs1_xfer_next) \/
-(ds_abs1.ds_abs1_xfer.state = abs1_xfer_next_write) \/
-(ds_abs1.ds_abs1_xfer.state = abs1_xfer_ready_for_reset))`
+((ds_abs1.state = abs1_xfer_idle) \/
+(ds_abs1.state = abs1_xfer_data) \/
+(ds_abs1.state = abs1_xfer_update))`
 
 (* DRIVER_ABS1_XFER_ENABLE: ds_abs1_state -> bool *)
 val DRIVER_ABS1_XFER_ENABLE_def = Define `
 DRIVER_ABS1_XFER_ENABLE (ds_abs1:ds_abs1_state) =
-((ds_abs1.ds_abs1_xfer.state = abs1_xfer_prepare) \/
-(ds_abs1.ds_abs1_xfer.state = abs1_xfer_ready) \/
-(ds_abs1.ds_abs1_xfer.state = abs1_xfer_fetch_data) \/
-(ds_abs1.ds_abs1_xfer.state = abs1_xfer_next) \/
-(ds_abs1.ds_abs1_xfer.state = abs1_xfer_done))`
+((ds_abs1.state = abs1_xfer_prepare) \/
+(ds_abs1.state = abs1_xfer_ready) \/
+(ds_abs1.state = abs1_xfer_fetch_data))`
 
 (* COMB_ABS1_XFER_ENABLE: ds_abs1_state -> bool *)
 val COMB_ABS1_XFER_ENABLE_def = Define `
 COMB_ABS1_XFER_ENABLE (ds_abs1:ds_abs1_state) =
-((ds_abs1.ds_abs1_xfer.state = abs1_xfer_trans) \/
-(ds_abs1.ds_abs1_xfer.state = abs1_xfer_ready_for_reset) \/
-(ds_abs1.ds_abs1_xfer.state = abs1_xfer_reset))`
+((ds_abs1.state = abs1_xfer_trans) \/
+(ds_abs1.state = abs1_xfer_reset))`
+
 
 (* tau_spi related functions *)
 (* spi_abs1_xfer_idle_op: ds_abs1_state -> ds_abs1_state *)
 val spi_abs1_xfer_idle_op_def = Define `
 spi_abs1_xfer_idle_op (ds_abs1:ds_abs1_state) =
-ds_abs1 with ds_abs1_xfer := ds_abs1.ds_abs1_xfer with
-state := abs1_xfer_prepare`
+ds_abs1 with state := abs1_xfer_prepare`
 
 (* spi_abs1_xfer_data_op: ds_abs1_state -> ds_abs1_state *)
 val spi_abs1_xfer_data_op_def = Define `
 spi_abs1_xfer_data_op (ds_abs1:ds_abs1_state) =
-ds_abs1 with <| ds_abs1_xfer := ds_abs1.ds_abs1_xfer with 
-state := abs1_xfer_exchange;
+ds_abs1 with <| state := abs1_xfer_exchange; 
 spi_abs1 := ds_abs1.spi_abs1 with
-TX_SHIFT_REG := (EL (ds_abs1.ds_abs1_xfer.xfer_cur_length - 1) (ds_abs1.ds_abs1_xfer.xfer_dataOUT_buffer))|>`
+TX_SHIFT_REG := (EL (ds_abs1.ds_abs1_xfer.xfer_cur_length - 1) 
+(ds_abs1.ds_abs1_xfer.xfer_dataOUT_buffer))|>`
 
 (* spi_abs1_xfer_update_op: ds_abs1_state -> ds_abs1_state *)
 val spi_abs1_xfer_update_op_def = Define `
 spi_abs1_xfer_update_op (ds_abs1:ds_abs1_state) =
-ds_abs1 with ds_abs1_xfer := ds_abs1.ds_abs1_xfer with
-state := abs1_xfer_ready`
-
-(* spi_abs1_xfer_fetch_data_op: ds_abs1_state -> ds_abs1_state *)
-val spi_abs1_xfer_fetch_data_op_def = Define `
-spi_abs1_xfer_fetch_data_op (ds_abs1:ds_abs1_state) =
-ds_abs1 with ds_abs1_xfer := ds_abs1.ds_abs1_xfer with
-state := abs1_xfer_done`
-
-(* spi_abs1_xfer_next_op: ds_abs1_state -> ds_abs1_state *)
-val spi_abs1_xfer_next_op_def = Define `
-spi_abs1_xfer_next_op (ds_abs1:ds_abs1_state) =
-ds_abs1 with ds_abs1_xfer := ds_abs1.ds_abs1_xfer with
-state := abs1_xfer_prepare`
-
-(* spi_abs1_xfer_next_write_op: ds_abs1_state -> ds_abs1_state *)
-val spi_abs1_xfer_next_write_op_def = Define `
-spi_abs1_xfer_next_write_op (ds_abs1:ds_abs1_state) =
-ds_abs1 with ds_abs1_xfer := ds_abs1.ds_abs1_xfer with
-state := abs1_xfer_trans`
-
-(* spi_abs1_xfer_ready_for_reset_op: ds_abs1_state -> ds_abs1_state *)
-val spi_abs1_xfer_ready_for_reset_op_def = Define `
-spi_abs1_xfer_ready_for_reset_op (ds_abs1:ds_abs1_state) =
-ds_abs1 with ds_abs1_xfer := ds_abs1.ds_abs1_xfer with
-state := abs1_xfer_reset`
+ds_abs1 with state := abs1_xfer_ready`
 
 (* spi_abs1_xfer_operations: ds_abs1_state -> ds_abs1_state *)
 val spi_abs1_xfer_operations_def = Define `
 spi_abs1_xfer_operations (ds_abs1:ds_abs1_state) =
-case ds_abs1.ds_abs1_xfer.state of 
-  | abs1_xfer_not_ready => ds_abs1 with err := T
-  | abs1_xfer_pre => ds_abs1 with err := T
-  | abs1_xfer_idle => spi_abs1_xfer_idle_op ds_abs1
-  | abs1_xfer_prepare => ds_abs1 with err := T
-  | abs1_xfer_trans => ds_abs1 with err := T
-  | abs1_xfer_data => spi_abs1_xfer_data_op ds_abs1
-  | abs1_xfer_exchange => ds_abs1 with err := T
-  | abs1_xfer_update => spi_abs1_xfer_update_op ds_abs1
-  | abs1_xfer_ready => ds_abs1 with err := T
-  | abs1_xfer_fetch_data => spi_abs1_xfer_fetch_data_op ds_abs1
-  | abs1_xfer_next => spi_abs1_xfer_next_op ds_abs1
-  | abs1_xfer_next_write => spi_abs1_xfer_next_write_op ds_abs1
-  | abs1_xfer_done => ds_abs1 with err := T
-  | abs1_xfer_ready_fot_reset => spi_abs1_xfer_ready_for_reset_op ds_abs1
-  | abs1_xfer_reset => ds_abs1 with err := T`
+if (ds_abs1.state = abs1_xfer_idle) then
+(spi_abs1_xfer_idle_op ds_abs1)
+else if (ds_abs1.state = abs1_xfer_data) then
+(spi_abs1_xfer_data_op ds_abs1)
+else if (ds_abs1.state = abs1_xfer_update) then
+(spi_abs1_xfer_update_op ds_abs1)
+else ds_abs1 with err := T`
 
 
 (* tau_driver related functions *)
 (* driver_abs1_xfer_prepare_op: ds_abs1_state -> ds_abs1_state *)
 val driver_abs1_xfer_prepare_op_def = Define `
 driver_abs1_xfer_prepare_op (ds_abs1:ds_abs1_state) =
-ds_abs1 with ds_abs1_xfer := ds_abs1.ds_abs1_xfer with 
-state := abs1_xfer_trans`
+ds_abs1 with state := abs1_xfer_trans`
 
 (* driver_abs1_xfer_ready_op: ds_abs1_state -> ds_abs1_state *)
 val driver_abs1_xfer_ready_op_def = Define `
 driver_abs1_xfer_ready_op (ds_abs1:ds_abs1_state) =
-ds_abs1 with ds_abs1_xfer := ds_abs1.ds_abs1_xfer with 
-state := abs1_xfer_fetch_data`
+ds_abs1 with state := abs1_xfer_fetch_data`
 
 (* driver_abs1_xfer_fetch_data_op: ds_abs1_state -> ds_abs1_state *)
 val driver_abs1_xfer_fetch_data_op_def = Define `
 driver_abs1_xfer_fetch_data_op (ds_abs1:ds_abs1_state) =
-ds_abs1 with ds_abs1_xfer := ds_abs1.ds_abs1_xfer with 
-<| state := if ds_abs1.ds_abs1_xfer.xfer_cur_length < (LENGTH (ds_abs1.ds_abs1_xfer.xfer_dataOUT_buffer)) 
-   then abs1_xfer_next else abs1_xfer_ready_for_reset;
-   xfer_dataIN_buffer := ds_abs1.ds_abs1_xfer.xfer_dataIN_buffer ++ [ds_abs1.spi_abs1.RX_SHIFT_REG] |>`
-
-(* driver_abs1_xfer_next_op: ds_abs1_state -> ds_abs1_state *)
-val driver_abs1_xfer_next_op_def = Define `
-driver_abs1_xfer_next_op (ds_abs1:ds_abs1_state) =
-ds_abs1 with ds_abs1_xfer := ds_abs1.ds_abs1_xfer with
-state := abs1_xfer_next_write`
-
-(* driver_abs1_xfer_done_op: ds_abs1_state -> ds_abs1_state *)
-val driver_abs1_xfer_done_op_def = Define `
-driver_abs1_xfer_done_op (ds_abs1:ds_abs1_state) =
-ds_abs1 with ds_abs1_xfer := ds_abs1.ds_abs1_xfer with
-<| state := if ds_abs1.ds_abs1_xfer.xfer_cur_length < (LENGTH (ds_abs1.ds_abs1_xfer.xfer_dataOUT_buffer)) 
-   then abs1_xfer_prepare else abs1_xfer_reset;
-   xfer_dataIN_buffer := ds_abs1.ds_abs1_xfer.xfer_dataIN_buffer ++ [ds_abs1.spi_abs1.RX_SHIFT_REG] |>`
+ds_abs1 with <| ds_abs1_xfer := ds_abs1.ds_abs1_xfer with 
+xfer_dataIN_buffer := ds_abs1.ds_abs1_xfer.xfer_dataIN_buffer ++ [ds_abs1.spi_abs1.RX_SHIFT_REG];
+state := if ds_abs1.ds_abs1_xfer.xfer_cur_length < (LENGTH (ds_abs1.ds_abs1_xfer.xfer_dataOUT_buffer)) 
+then abs1_xfer_prepare else abs1_xfer_reset |>`
 
 (* driver_abs1_xfer_operations: ds_abs1_state -> ds_abs1_state *)
 val driver_abs1_xfer_operations_def = Define `
 driver_abs1_xfer_operations (ds_abs1:ds_abs1_state) =
-case ds_abs1.ds_abs1_xfer.state of
-  | abs1_xfer_not_ready => ds_abs1 with err := T
-  | abs1_xfer_pre => ds_abs1 with err := T
-  | abs1_xfer_idle => ds_abs1 with err := T
-  | abs1_xfer_prepare => driver_abs1_xfer_prepare_op ds_abs1
-  | abs1_xfer_trans => ds_abs1 with err := T
-  | abs1_xfer_data => ds_abs1 with err := T
-  | abs1_xfer_exchange => ds_abs1 with err := T
-  | abs1_xfer_update => ds_abs1 with err := T
-  | abs1_xfer_ready => driver_abs1_xfer_ready_op ds_abs1
-  | abs1_xfer_fetch_data => driver_abs1_xfer_fetch_data_op ds_abs1
-  | abs1_xfer_next => driver_abs1_xfer_next_op ds_abs1
-  | abs1_xfer_next_write => ds_abs1 with err := T
-  | abs1_xfer_done => driver_abs1_xfer_done_op ds_abs1
-  | abs1_xfer_ready_for_reset => ds_abs1 with err := T
-  | abs1_xfer_reset => ds_abs1 with err := T`
+if (ds_abs1.state = abs1_xfer_prepare) then
+(driver_abs1_xfer_prepare_op ds_abs1)
+else if (ds_abs1.state = abs1_xfer_ready) then
+(driver_abs1_xfer_ready_op ds_abs1)
+else if (ds_abs1.state = abs1_xfer_fetch_data) then
+(driver_abs1_xfer_fetch_data_op ds_abs1)
+else ds_abs1 with err := T`
 
 
 (* tau_comb related functions *)
 (* comb_abs1_xfer_trans_op: ds_abs1_state -> ds_abs1_state *)
 val comb_abs1_xfer_trans_op_def = Define `
 comb_abs1_xfer_trans_op (ds_abs1:ds_abs1_state) =
-ds_abs1 with ds_abs1_xfer := ds_abs1.ds_abs1_xfer with
-<| state := abs1_xfer_data;
-   xfer_cur_length := ds_abs1.ds_abs1_xfer.xfer_cur_length + 1 |>`
-
-(* comb_abs1_xfer_ready_for_reset_op: ds_abs1_state -> ds_abs1_state *)
-val comb_abs1_xfer_ready_for_reset_op_def = Define `
-comb_abs1_xfer_ready_for_reset_op (ds_abs1:ds_abs1_state) =
-ds_abs1 with ds_abs1_xfer := ds_abs1.ds_abs1_xfer with 
-state := abs1_xfer_reset`
+ds_abs1 with <| ds_abs1_xfer := ds_abs1.ds_abs1_xfer with 
+xfer_cur_length := ds_abs1.ds_abs1_xfer.xfer_cur_length + 1;
+state := abs1_xfer_data |>`
 
 (* comb_abs1_xfer_reset_op: ds_abs1_state -> ds_abs1_state *)
 val comb_abs1_xfer_reset_op_def = Define `
 comb_abs1_xfer_reset_op (ds_abs1:ds_abs1_state) =
-ds_abs1 with ds_abs1_xfer := ds_abs1.ds_abs1_xfer with
-state := abs1_xfer_pre`
+ds_abs1 with state := abs1_ready`
 
 (* comb_abs1_xfer_operations: ds_abs1_state -> ds_abs1_state *)
 val comb_abs1_xfer_operations_def = Define `
 comb_abs1_xfer_operations (ds_abs1:ds_abs1_state) =
-if ds_abs1.ds_abs1_xfer.state = abs1_xfer_trans 
+if ds_abs1.state = abs1_xfer_trans 
 then (comb_abs1_xfer_trans_op ds_abs1)
-else if ds_abs1.ds_abs1_xfer.state = abs1_xfer_ready_for_reset
-then (comb_abs1_xfer_ready_for_reset_op ds_abs1)
-else if ds_abs1.ds_abs1_xfer.state = abs1_xfer_reset
+else if (ds_abs1.state = abs1_xfer_reset)
 then (comb_abs1_xfer_reset_op ds_abs1)
 else ds_abs1 with err := T`
 
@@ -191,10 +115,10 @@ val abs1_xfer_exchange_op_def = Define `
 abs1_xfer_exchange_op (ds_abs1:ds_abs1_state) (data: word8 option) =
 if (data <> NONE) then
 (ds_abs1 with
-<| ds_abs1_xfer := ds_abs1.ds_abs1_xfer with state := abs1_xfer_update;
+<| state := abs1_xfer_update;
    spi_abs1 := ds_abs1.spi_abs1 with RX_SHIFT_REG := THE data |>,
 SOME ds_abs1.spi_abs1.TX_SHIFT_REG)
-else (ds_abs1, NONE)`
+else (ds_abs1 with err := T, NONE)`
 
 (* abs1_xfer_exchange_op_value: ds_abs1_state -> word8 option -> ds_abs1_state *)
 val abs1_xfer_exchange_op_value_def = Define `
@@ -211,10 +135,10 @@ ds_abs1'`
 (* call_xfer_ds_abs1: ds_abs1_state -> word8 list -> ds_abs1_state *)
 val call_xfer_ds_abs1_def = Define `
 call_xfer_ds_abs1 (ds_abs1:ds_abs1_state) (buffer:word8 list) =
-ds_abs1 with ds_abs1_xfer := ds_abs1.ds_abs1_xfer with
-<| state := abs1_xfer_idle;
-   xfer_dataOUT_buffer := buffer;
+ds_abs1 with <| ds_abs1_xfer := ds_abs1.ds_abs1_xfer with
+<| xfer_dataOUT_buffer := buffer;
    xfer_dataIN_buffer := [];
-   xfer_cur_length := 0 |>`
+   xfer_cur_length := 0 |>;
+state := abs1_xfer_idle |>`
 
 val _ = export_theory();
