driver_model/driver_callScript.sml
@@ -6,31 +6,25 @@ val _ = new_theory "driver_call";
 (* call_init_dr: driver_state -> driver_state *)
 val call_init_dr_def = Define `
 call_init_dr (dr:driver_state) =
-dr with dr_init := dr.dr_init with state := dr_init_idle`
+dr with state := dr_init_idle`
 
 (* call_tx_dr: driver_state -> word8 list -> driver_state *)
 val call_tx_dr_def = Define `
 call_tx_dr (dr:driver_state) (buffer:word8 list) =
-dr with dr_tx := dr.dr_tx with
-<| state := dr_tx_idle;
-data_buf := buffer;
-tx_cur_length := 0 |>`
+dr with <| dr_tx := dr.dr_tx with <| tx_data_buf := buffer; tx_cur_length := 0 |>;
+state := dr_tx_idle |>`
 
 (* call_rx_dr: driver_state -> num -> driver_state *)
 val call_rx_dr_def = Define `
 call_rx_dr (dr:driver_state) (length: num) =
-dr with dr_rx := dr.dr_rx with
-<| state := dr_rx_idle;
-rx_left_length := length;
-rx_data_buf := [] |>`
+dr with <| dr_rx := dr.dr_rx with <| rx_left_length := length; rx_data_buf := [] |>;
+state := dr_rx_idle |>`
 
 (* call_xfer_dr: driver_state -> word8 list -> driver_state *)
 val call_xfer_dr_def = Define `
 call_xfer_dr (dr:driver_state) (buffer:word8 list) =
-dr with dr_xfer := dr.dr_xfer with
-<| state := dr_xfer_idle;
-xfer_dataOUT_buf := buffer;
-xfer_dataIN_buf := [];
-xfer_cur_length := 0 |>`
+dr with <| dr_xfer := dr.dr_xfer with <| xfer_dataOUT_buf := buffer; xfer_dataIN_buf := [];
+xfer_cur_length := 0 |>;
+state := dr_xfer_idle |>`
 
 val _ = export_theory();
