driver_model/driver_readScript.sml
@@ -5,94 +5,92 @@ open driver_stateTheory board_memTheory;
 (* Driver issues a read request to the SPI controller, mainly update dr.dr_last_read_ad *)
 val _ = new_theory "driver_read";
 
+(* DR_RD_ENABLE: driver_state -> bool *)
+val DR_RD_ENABLE_def = Define ` 
+DR_RD_ENABLE (dr:driver_state) =
+(dr.state = dr_init_read_req \/
+dr.state = dr_tx_read_txs \/
+dr.state = dr_tx_read_eot \/
+dr.state = dr_rx_read_rxs \/
+dr.state = dr_rx_read_rx0 \/
+dr.state = dr_xfer_read_txs \/
+dr.state = dr_xfer_read_rxs \/
+dr.state = dr_xfer_read_rx0)`
+
 (* dr_read_sysstatus: driver_state -> driver_state *)
 val dr_read_sysstatus_def = Define `
 dr_read_sysstatus (dr:driver_state) =
-case dr.dr_init.state of
-  | dr_init_pre => dr with dr_last_read_ad := NONE
-  | dr_init_idle => dr with dr_last_read_ad := NONE
-  | dr_init_read_req => 
-    dr with <| dr_init := dr.dr_init with state := dr_init_check_rep;
-    dr_last_read_ad := SOME SPI0_SYSSTATUS |>
-  | dr_init_check_rep => dr with dr_last_read_ad := NONE
-  | dr_init_setting => dr with dr_last_read_ad := NONE
-  | dr_init_done => dr with dr_last_read_ad := NONE`
+dr with <| state := dr_init_check_rep;
+dr_last_read_ad := SOME SPI0_SYSSTATUS |>`
 
 (* dr_read_ch0stat: driver_state -> driver_state *)
 val dr_read_ch0stat_def = Define `
 dr_read_ch0stat (dr:driver_state) =
-if (dr.dr_init.state = dr_init_done) /\ (dr.dr_tx.state = dr_tx_read_txs) /\
-   (dr.dr_rx.state = dr_rx_idle) /\ (dr.dr_xfer.state = dr_xfer_idle) then
-   dr with <| dr_tx := dr.dr_tx with state := dr_tx_check_txs;
-   dr_last_read_ad := SOME SPI0_CH0STAT |>
-else if (dr.dr_init.state = dr_init_done) /\ (dr.dr_tx.state = dr_tx_read_eot) /\
-   (dr.dr_rx.state = dr_rx_idle) /\ (dr.dr_xfer.state = dr_xfer_idle) then
-   dr with <| dr_tx := dr.dr_tx with state := dr_tx_check_eot;
-   dr_last_read_ad := SOME SPI0_CH0STAT |>
-else if (dr.dr_init.state = dr_init_done) /\ (dr.dr_tx.state = dr_tx_idle) /\
-   (dr.dr_rx.state = dr_rx_read_rxs) /\ (dr.dr_xfer.state = dr_xfer_idle) then
-   dr with <| dr_rx := dr.dr_rx with state := dr_rx_check_rxs;
-   dr_last_read_ad := SOME SPI0_CH0STAT |>
-else if (dr.dr_init.state = dr_init_done) /\ (dr.dr_tx.state = dr_tx_idle) /\
-   (dr.dr_rx.state = dr_rx_idle) /\ (dr.dr_xfer.state = dr_xfer_read_txs) then
-   dr with <| dr_xfer := dr.dr_xfer with state := dr_xfer_check_txs;
-   dr_last_read_ad := SOME SPI0_CH0STAT |>
-else if (dr.dr_init.state = dr_init_done) /\ (dr.dr_tx.state = dr_tx_idle) /\
-   (dr.dr_rx.state = dr_rx_idle) /\ (dr.dr_xfer.state = dr_xfer_read_rxs) then
-   dr with <| dr_xfer := dr.dr_xfer with state := dr_xfer_check_rxs;
-   dr_last_read_ad := SOME SPI0_CH0STAT |>
-else dr with dr_last_read_ad := NONE`
+if (dr.state = dr_tx_read_txs) then 
+dr with <| state := dr_tx_check_txs;
+dr_last_read_ad := SOME SPI0_CH0STAT |>
+else if (dr.state = dr_tx_read_eot) then
+dr with <| state := dr_tx_check_eot;
+dr_last_read_ad := SOME SPI0_CH0STAT |>
+else if (dr.state = dr_rx_read_rxs) then
+dr with <| state := dr_rx_check_rxs;
+dr_last_read_ad := SOME SPI0_CH0STAT |>
+else if (dr.state = dr_xfer_read_txs) then
+dr with <| state := dr_xfer_check_txs; 
+dr_last_read_ad := SOME SPI0_CH0STAT |>
+else if (dr.state = dr_xfer_read_rxs) then
+dr with <| state := dr_xfer_check_rxs;
+dr_last_read_ad := SOME SPI0_CH0STAT |>
+else dr with dr_err := T`
 
 (* dr_read_rx0: driver_state ->  driver_state *)
 val dr_read_rx0_def = Define `
 dr_read_rx0 (dr:driver_state) =
-if (dr.dr_rx.state = dr_rx_read_rx0) 
-then dr with <| dr_rx := dr.dr_rx with state := dr_rx_fetch_data;
-   dr_last_read_ad := SOME SPI0_RX0 |>
-else if (dr.dr_xfer.state = dr_xfer_read_rx0) 
-then dr with <| dr_xfer := dr.dr_xfer with state := dr_xfer_fetch_dataI;
-   dr_last_read_ad := SOME SPI0_RX0 |>
-else dr with dr_last_read_ad := NONE`
-
-(* INIT_RD_ENABLE: driver_state -> bool *)
-val INIT_RD_ENABLE_def = Define ` 
-INIT_RD_ENABLE (dr:driver_state) =
-(dr.dr_init.state = dr_init_read_req)`
-
-(* TX_RD_ENABLE: driver_state -> bool *)
-val TX_RD_ENABLE_def = Define `
-TX_RD_ENABLE (dr:driver_state) =
-(dr.dr_tx.state = dr_tx_read_txs \/
- dr.dr_tx.state = dr_tx_read_eot)`
-
-(* RX_RD_ENABLE: driver_state -> bool *)
-val RX_RD_ENABLE_def = Define `
-RX_RD_ENABLE (dr:driver_state) =
-(dr.dr_rx.state = dr_rx_read_rxs \/
- dr.dr_rx.state = dr_rx_read_rx0)`
-
-(* XFER_RD_ENABLE: driver_state -> bool *)
-val XFER_RD_ENABLE_def = Define `
-XFER_RD_ENABLE (dr:driver_state) =
-(dr.dr_xfer.state = dr_xfer_read_txs \/
- dr.dr_xfer.state = dr_xfer_read_rxs \/ 
- dr.dr_xfer.state = dr_xfer_read_rx0)`
+if (dr.state = dr_rx_read_rx0) then 
+dr with <| state := dr_rx_fetch_data;
+dr_last_read_ad := SOME SPI0_RX0 |>
+else if (dr.state = dr_xfer_read_rx0) then 
+dr with <| state := dr_xfer_fetch_dataI;
+dr_last_read_ad := SOME SPI0_RX0 |>
+else dr with dr_err := T`
 
 (* dr_read: driver_state -> driver_state *)
 val dr_read_def = Define `
 dr_read (dr:driver_state) =
-if dr.dr_err then dr with dr_last_read_ad := NONE
-else if (INIT_RD_ENABLE dr) then (dr_read_sysstatus dr)
-else if (TX_RD_ENABLE dr) /\ (dr.dr_tx.state = dr_tx_read_txs \/ dr.dr_tx.state = dr_tx_read_eot)
-then (dr_read_ch0stat dr)
-else if (RX_RD_ENABLE dr) /\ (dr.dr_rx.state = dr_rx_read_rxs)
-then (dr_read_ch0stat dr)
-else if (RX_RD_ENABLE dr) /\ (dr.dr_rx.state = dr_rx_read_rx0)
-then (dr_read_rx0 dr)
-else if (XFER_RD_ENABLE dr) /\ (dr.dr_xfer.state = dr_xfer_read_txs \/ dr.dr_xfer.state = dr_xfer_read_rxs)
-then (dr_read_ch0stat dr)
-else if (XFER_RD_ENABLE dr) /\ (dr.dr_xfer.state = dr_xfer_read_rx0)
-then (dr_read_rx0 dr)
-else dr with dr_last_read_ad := NONE`
+case dr.state of
+  | dr_init_pre => dr with dr_err := T
+  | dr_init_idle => dr with dr_err := T  
+  | dr_init_read_req => (dr_read_sysstatus dr)
+  | dr_init_check_rep => dr with dr_err := T
+  | dr_init_setting => dr with dr_err := T
+  | dr_ready => dr with dr_err := T
+  | dr_tx_idle => dr with dr_err := T
+  | dr_tx_conf_issued => dr with dr_err := T
+  | dr_tx_read_txs => (dr_read_ch0stat dr)
+  | dr_tx_check_txs => dr with dr_err := T
+  | dr_tx_write_data => dr with dr_err := T
+  | dr_tx_read_eot => (dr_read_ch0stat dr)
+  | dr_tx_check_eot => dr with dr_err := T
+  | dr_tx_issue_disable => dr with dr_err := T
+  | dr_tx_reset_conf => dr with dr_err := T
+  | dr_rx_idle => dr with dr_err := T
+  | dr_rx_conf_issued => dr with dr_err := T
+  | dr_rx_read_rxs => (dr_read_ch0stat dr)
+  | dr_rx_check_rxs => dr with dr_err := T
+  | dr_rx_read_rx0 => (dr_read_rx0 dr)
+  | dr_rx_fetch_data => dr with dr_err := T
+  | dr_rx_issue_disable => dr with dr_err := T
+  | dr_rx_reset_conf => dr with dr_err := T
+  | dr_xfer_idle => dr with dr_err := T
+  | dr_xfer_conf_issued => dr with dr_err := T
+  | dr_xfer_read_txs => (dr_read_ch0stat dr)
+  | dr_xfer_check_txs => dr with dr_err := T
+  | dr_xfer_write_dataO => dr with dr_err := T
+  | dr_xfer_read_rxs => (dr_read_ch0stat dr)
+  | dr_xfer_check_rxs => dr with dr_err := T
+  | dr_xfer_read_rx0 => (dr_read_rx0 dr)
+  | dr_xfer_fetch_dataI => dr with dr_err := T
+  | dr_xfer_issue_disable => dr with dr_err := T
+  | dr_xfer_reset_conf => dr with dr_err := T`
 
 val _ = export_theory();
