driver_model/driver_stateScript.sml
@@ -5,54 +5,41 @@ open wordsLib wordsTheory;
 val _ = new_theory "driver_state";
 
 (* driver_state *)
-(* dr_init_general_state: spi driver initiliztion fucntion state flags *)
-val _ = Datatype `dr_init_general_state =
+(* dr_general_state: spi driver general states *)
+val _ = Datatype `dr_general_state =
 | dr_init_pre | dr_init_idle | dr_init_read_req 
-| dr_init_check_rep | dr_init_setting | dr_init_done`
+| dr_init_check_rep | dr_init_setting | dr_ready
+| dr_tx_idle | dr_tx_conf_issued | dr_tx_read_txs 
+| dr_tx_check_txs | dr_tx_write_data | dr_tx_read_eot 
+| dr_tx_check_eot | dr_tx_issue_disable | dr_tx_reset_conf
+| dr_rx_idle | dr_rx_conf_issued | dr_rx_read_rxs 
+| dr_rx_check_rxs | dr_rx_read_rx0 | dr_rx_fetch_data 
+| dr_rx_issue_disable | dr_rx_reset_conf
+| dr_xfer_idle | dr_xfer_conf_issued | dr_xfer_read_txs 
+| dr_xfer_check_txs | dr_xfer_write_dataO | dr_xfer_read_rxs 
+| dr_xfer_check_rxs | dr_xfer_read_rx0 | dr_xfer_fetch_dataI 
+| dr_xfer_issue_disable | dr_xfer_reset_conf`
 
-(* dr_init_state *)
+(* dr_init_state: contains boolean flags to record init process *)
 val _ = Datatype `dr_init_state = <|
-state: dr_init_general_state;
 issue_wr_sysconfig: bool;
 issue_wr_modulctrl: bool;
 issue_wr_ch0conf_wl: bool;
 issue_wr_ch0conf_mode: bool;
 issue_wr_ch0conf_speed: bool |>`
 
-(* dr_tx_general_state: spi driver transimit function state flags *)
-val _ = Datatype ` dr_tx_general_state =
-| dr_tx_not_ready | dr_tx_pre | dr_tx_idle | dr_tx_conf_issued | dr_tx_read_txs 
-| dr_tx_check_txs | dr_tx_write_data | dr_tx_read_eot 
-| dr_tx_check_eot | dr_tx_issue_disable | dr_tx_reset_conf`
-
-(* dr_tx_state *)
+(* dr_tx_state: include the transimit buffer and length *)
 val _ = Datatype `dr_tx_state = <|
-state: dr_tx_general_state; 
-data_buf: word8 list;
+tx_data_buf: word8 list;
 tx_cur_length: num |>`
 
-(* dr_rx_general_state: spi driver receive function state flags *)
-val _ = Datatype `dr_rx_general_state = 
-| dr_rx_not_ready | dr_rx_pre | dr_rx_idle | dr_rx_conf_issued | dr_rx_read_rxs 
-| dr_rx_check_rxs | dr_rx_read_rx0 | dr_rx_fetch_data 
-| dr_rx_issue_disable | dr_rx_reset_conf`
-
-(* dr_rx_state *)
+(* dr_rx_state: include the receive buffer and length *)
 val _ = Datatype `dr_rx_state = <|
-state: dr_rx_general_state;
 rx_data_buf : word8 list;
 rx_left_length: num |>`
 
-(* dr_xfer_general_state: spi driver transfer(full-duplex) function state flags *)
-val _ = Datatype `dr_xfer_general_state =
-| dr_xfer_not_ready | dr_xfer_pre | dr_xfer_idle | dr_xfer_conf_issued 
-| dr_xfer_read_txs | dr_xfer_check_txs | dr_xfer_write_dataO 
-| dr_xfer_read_rxs | dr_xfer_check_rxs | dr_xfer_read_rx0 
-| dr_xfer_fetch_dataI | dr_xfer_issue_disable | dr_xfer_reset_conf`
-
-(* dr_xfer_state *)
+(* dr_xfer_state: include the two data buffers for transmitting and receiving, and the length *)
 val _ = Datatype `dr_xfer_state = <|
-state: dr_xfer_general_state;
 xfer_dataIN_buf: word8 list;
 xfer_dataOUT_buf: word8 list;
 xfer_cur_length : num |>`
@@ -60,18 +47,12 @@ xfer_cur_length : num |>`
 (* driver_state: spi driver state, including init, tx, rx and xfer functions state *)
 val _ = Datatype `driver_state = <|
 dr_err: bool;
+state: dr_general_state;
 dr_last_read_ad: word32 option;
 dr_last_read_v: word32 option;
 dr_init: dr_init_state;
 dr_tx: dr_tx_state;
 dr_rx: dr_rx_state;
 dr_xfer: dr_xfer_state |>`
-
-(* Datatypes for driver synchronzing labels *)
-val _ = Datatype `dr_tx_syn_lbl_type = | DR_TX_SYN_RD | DR_TX_SYN_NRD `
-
-val _ = Datatype `dr_rx_syn_lbl_type = | DR_RX_SYN_RD | DR_RX_SYN_NRD `
-
-val _ = Datatype `dr_xfer_syn_lbl_type = | DR_XFER_SYN_RD | DR_XFER_SYN_NRD ` 
 
 val _ = export_theory();
