driver_model/driver_writeScript.sml
@@ -5,110 +5,93 @@ open driver_stateTheory board_memTheory;
 (* Driver issues a write request to the SPI controller *)
 val _ = new_theory "driver_write";
 
+(* Driver is available to issue write commands.
+ * DR_WR_ENABLE:driver_state -> bool
+ *)
+val DR_WR_ENABLE_def = Define `
+DR_WR_ENABLE (dr:driver_state) =
+(dr.state = dr_init_idle \/
+dr.state = dr_init_setting \/ 
+dr.state = dr_tx_idle \/
+dr.state = dr_tx_conf_issued \/ 
+dr.state = dr_tx_write_data \/
+dr.state = dr_tx_issue_disable \/
+dr.state = dr_tx_reset_conf \/
+dr.state = dr_rx_idle \/
+dr.state = dr_rx_conf_issued \/
+dr.state = dr_rx_issue_disable \/
+dr.state = dr_rx_reset_conf \/
+dr.state = dr_xfer_idle \/
+dr.state = dr_xfer_conf_issued \/
+dr.state = dr_xfer_write_dataO \/
+dr.state = dr_xfer_issue_disable \/
+dr.state = dr_xfer_reset_conf)`
+
 (* dr_write_softreset: driver_state -> word32 option * word32 option * driver_state *)
 val dr_write_softreset_def = Define `
 dr_write_softreset (dr:driver_state) =
 let addr = SPI0_SYSCONFIG:word32 and
-    v = 0x00000002w:word32 in
-case dr.dr_init.state of
-  | dr_init_idle => (SOME addr, SOME v, 
-    dr with dr_init := dr.dr_init with <|state := dr_init_read_req;
-    issue_wr_sysconfig := F; issue_wr_modulctrl := F; issue_wr_ch0conf_wl := F;
-    issue_wr_ch0conf_mode := F; issue_wr_ch0conf_speed := F |>)
-  | dr_init_read_req => (NONE, NONE, dr)
-  | dr_init_check_rep => (NONE, NONE, dr)
-  | dr_init_setting => (NONE, NONE, dr)
-  | dr_init_done => (NONE, NONE, dr)`
+    v = 0x00000002w:word32 in 
+(SOME addr, SOME v, 
+dr with <| dr_init := dr.dr_init with <|issue_wr_sysconfig := F; 
+issue_wr_modulctrl := F; issue_wr_ch0conf_wl := F;
+issue_wr_ch0conf_mode := F; issue_wr_ch0conf_speed := F |>;
+state := dr_init_read_req |>)`
 
 (* dr_write_sysconfig: driver_state -> word32 option * word32 option * driver_state *)
 val dr_write_sysconfig_def = Define `
 dr_write_sysconfig (dr:driver_state) =
 let addr = SPI0_SYSCONFIG:word32 and
-    v = 0x00000011w:word32 in
-case dr.dr_init.state of
-  | dr_init_idle => (NONE, NONE, dr)
-  | dr_init_read_req => (NONE, NONE, dr)
-  | dr_init_check_rep => (NONE, NONE, dr)
-  | dr_init_setting => (SOME addr, SOME v,
-    dr with <| dr_init := dr.dr_init with <|
-    issue_wr_sysconfig := T;
-    state := 
-    if (dr.dr_init.issue_wr_modulctrl) /\ (dr.dr_init.issue_wr_ch0conf_wl)
-    /\ (dr.dr_init.issue_wr_ch0conf_mode) /\ (dr.dr_init.issue_wr_ch0conf_speed) 
-    then dr_init_done else dr_init_setting |> |>)
-  | dr_init_done => (NONE, NONE, dr)`
+    v = 0x00000011w:word32 in 
+(SOME addr, SOME v,
+dr with <| dr_init := dr.dr_init with issue_wr_sysconfig := T;
+state := if (dr.dr_init.issue_wr_modulctrl) /\ (dr.dr_init.issue_wr_ch0conf_wl) /\ 
+(dr.dr_init.issue_wr_ch0conf_mode) /\ (dr.dr_init.issue_wr_ch0conf_speed) 
+then dr_ready else dr_init_setting |>)`
 
 (* dr_write_modulctrl: driver_state -> word32 option * word32 option * driver_state *)
 val dr_write_modulctrl_def = Define `
 dr_write_modulctrl (dr:driver_state) =
 let addr = SPI0_MODULCTRL:word32 and
     v = 0x00000001w:word32 in
-case dr.dr_init.state of
-  | dr_init_idle => (NONE, NONE, dr)
-  | dr_init_read_req => (NONE, NONE, dr)
-  | dr_init_check_rep => (NONE, NONE, dr)
-  | dr_init_setting => (SOME addr, SOME v,
-    dr with <| dr_init := dr.dr_init with <|
-    issue_wr_modulctrl := T;
-    state :=  
-    if (dr.dr_init.issue_wr_sysconfig) /\ (dr.dr_init.issue_wr_ch0conf_wl) 
-    /\ (dr.dr_init.issue_wr_ch0conf_mode) /\ (dr.dr_init.issue_wr_ch0conf_speed) 
-    then dr_init_done else dr_init_setting |> |>)
-  | dr_init_done => (NONE, NONE, dr)`
+(SOME addr, SOME v,
+dr with <| dr_init := dr.dr_init with issue_wr_modulctrl := T;
+state := if (dr.dr_init.issue_wr_sysconfig) /\ (dr.dr_init.issue_wr_ch0conf_wl) /\ 
+(dr.dr_init.issue_wr_ch0conf_mode) /\ (dr.dr_init.issue_wr_ch0conf_speed) 
+then dr_ready else dr_init_setting |>)`
 
 (* dr_write_ch0conf_wl: driver_state -> word32 option * word32 option * driver_state *)
 val dr_write_ch0conf_wl_def = Define `
 dr_write_ch0conf_wl (dr:driver_state) =
 let addr = SPI0_CH0CONF:word32 and
     v = 0x00000380w:word32 in
-case dr.dr_init.state of
-  | dr_init_idle => (NONE, NONE, dr)
-  | dr_init_read_req => (NONE, NONE, dr)
-  | dr_init_check_rep => (NONE, NONE, dr)
-  | dr_init_setting => (SOME addr, SOME v,
-    dr with <| dr_init := dr.dr_init with <|
-    issue_wr_ch0conf_wl := T;
-    state :=  
-    if (dr.dr_init.issue_wr_sysconfig) /\ (dr.dr_init.issue_wr_modulctrl) /\
-    (dr.dr_init.issue_wr_ch0conf_mode) /\ (dr.dr_init.issue_wr_ch0conf_speed)
-    then dr_init_done else dr_init_setting |> |>)
-  | dr_init_done => (NONE, NONE, dr)`
+(SOME addr, SOME v,
+dr with <| dr_init := dr.dr_init with issue_wr_ch0conf_wl := T;
+state :=  if (dr.dr_init.issue_wr_sysconfig) /\ (dr.dr_init.issue_wr_modulctrl) /\
+(dr.dr_init.issue_wr_ch0conf_mode) /\ (dr.dr_init.issue_wr_ch0conf_speed)
+then dr_ready else dr_init_setting |>)`
 
 (* dr_write_ch0conf_mode: driver_state -> word32 option * word32 option * driver_state *)
 val dr_write_ch0conf_mode_def = Define `
 dr_write_ch0conf_mode (dr:driver_state) =
 let addr = SPI0_CH0CONF:word32 and
     v = 0x00010040w:word32 in
-case dr.dr_init.state of
-  | dr_init_idle => (NONE, NONE, dr)
-  | dr_init_read_req => (NONE, NONE, dr)
-  | dr_init_check_rep => (NONE, NONE, dr)   
-  | dr_init_setting => (SOME addr, SOME v,
-    dr with <| dr_init := dr.dr_init with <|
-    issue_wr_ch0conf_mode := T;
-    state :=  
-    if (dr.dr_init.issue_wr_sysconfig) /\ (dr.dr_init.issue_wr_modulctrl) /\
-    (dr.dr_init.issue_wr_ch0conf_wl) /\ (dr.dr_init.issue_wr_ch0conf_speed) 
-    then dr_init_done else dr_init_setting |> |>)
-  | dr_init_done => (NONE, NONE, dr)`
+(SOME addr, SOME v,
+dr with <| dr_init := dr.dr_init with issue_wr_ch0conf_mode := T;
+state :=  if (dr.dr_init.issue_wr_sysconfig) /\ (dr.dr_init.issue_wr_modulctrl) /\
+(dr.dr_init.issue_wr_ch0conf_wl) /\ (dr.dr_init.issue_wr_ch0conf_speed) 
+then dr_ready else dr_init_setting |>)`
 
 (* dr_write_ch0conf_speed: driver_state -> word32 option * word32 option * driver_state *)
 val dr_write_ch0conf_speed_def = Define `
 dr_write_ch0conf_speed (dr:driver_state) =
 let addr = SPI0_CH0CONF:word32 and
     v = 0x00000018w:word32 in
-case dr.dr_init.state of
-  | dr_init_idle => (NONE, NONE, dr)
-  | dr_init_read_req => (NONE, NONE, dr)
-  | dr_init_check_rep => (NONE, NONE, dr)   
-  | dr_init_setting => (SOME addr, SOME v,
-    dr with <| dr_init := dr.dr_init with <|
-    issue_wr_ch0conf_speed := T;
-    state :=  
-    if (dr.dr_init.issue_wr_sysconfig) /\ (dr.dr_init.issue_wr_modulctrl) /\
-    (dr.dr_init.issue_wr_ch0conf_wl) /\ (dr.dr_init.issue_wr_ch0conf_mode) 
-    then dr_init_done else dr_init_setting |> |>)
-  | dr_init_done => (NONE, NONE, dr)`
+(SOME addr, SOME v,
+dr with <| dr_init := dr.dr_init with issue_wr_ch0conf_speed := T;
+state :=  if (dr.dr_init.issue_wr_sysconfig) /\ (dr.dr_init.issue_wr_modulctrl) /\ 
+(dr.dr_init.issue_wr_ch0conf_wl) /\ (dr.dr_init.issue_wr_ch0conf_mode) 
+then dr_ready else dr_init_setting |>)`
 
 (* dr_write_ch0conf_tx: driver_state -> word32 option * word32 option * driver_state *)
 val dr_write_ch0conf_tx_def = Define `
@@ -116,21 +99,11 @@ dr_write_ch0conf_tx (dr:driver_state) =
 let addr = SPI0_CH0CONF:word32 and
     v1 = 0x00102000w:word32 and
     v2 = 0x00000000w:word32 in
-case dr.dr_tx.state of
-  | dr_tx_not_ready => (NONE, NONE, dr)
-  | dr_tx_pre => (NONE, NONE, dr)
-  | dr_tx_idle => 
-    (SOME addr, SOME v1, 
-    dr with dr_tx := dr.dr_tx with state := dr_tx_conf_issued )
-  | dr_tx_conf_issued => (NONE, NONE, dr)
-  | dr_tx_read_txs => (NONE, NONE, dr) 
-  | dr_tx_check_txs => (NONE, NONE, dr)
-  | dr_tx_write_data => (NONE, NONE, dr)
-  | dr_tx_read_eot => (NONE, NONE, dr)
-  | dr_tx_check_eot => (NONE, NONE, dr)    
-  | dr_tx_issue_disable => (NONE, NONE, dr)
-  | dr_tx_reset_conf => (SOME addr, SOME v2,
-    dr with dr_tx := dr.dr_tx with state := dr_tx_pre)`
+if (dr.state = dr_tx_idle) then
+(SOME addr, SOME v1, dr with state := dr_tx_conf_issued)
+else if (dr.state = dr_tx_reset_conf) then 
+(SOME addr, SOME v2, dr with state := dr_ready)
+else (NONE, NONE, dr with dr_err := T)`
 
 (* dr_write_ch0conf_rx: driver_state -> word32 option * word32 option * driver_state *)
 val dr_write_ch0conf_rx_def = Define `
@@ -138,20 +111,11 @@ dr_write_ch0conf_rx (dr:driver_state) =
 let addr = SPI0_CH0CONF:word32 and
     v1 = 0x00101000w:word32 and
     v2 = 0x00000000w:word32 in
-case dr.dr_rx.state of
-  | dr_rx_not_ready => (NONE, NONE, dr)
-  | dr_rx_pre => (NONE, NONE, dr)
-  | dr_rx_idle => (SOME addr, SOME v1, 
-    dr with dr_rx := dr.dr_rx with
-    state := dr_rx_conf_issued )
-  | dr_rx_conf_issued => (NONE, NONE, dr)
-  | dr_rx_read_rxs => (NONE, NONE, dr)
-  | dr_rx_check_rxs => (NONE, NONE, dr)
-  | dr_rx_read_rx0 => (NONE, NONE, dr)
-  | dr_rx_fetch_data => (NONE, NONE, dr)
-  | dr_rx_issue_disable => (NONE, NONE, dr)
-  | dr_rx_reset_conf => (SOME addr, SOME v2,
-    dr with dr_rx := dr.dr_rx with state := dr_rx_pre)`
+if (dr.state = dr_rx_idle) then
+(SOME addr, SOME v1, dr with state := dr_rx_conf_issued)
+else if (dr.state = dr_rx_reset_conf) then
+(SOME addr, SOME v2, dr with state := dr_ready)
+else (NONE, NONE, dr with dr_err := T)`
 
 (* dr_write_ch0conf_xfer: driver_state -> word32 option * word32 option * driver_state *)
 val dr_write_ch0conf_xfer_def = Define `
@@ -159,156 +123,108 @@ dr_write_ch0conf_xfer (dr:driver_state) =
 let addr = SPI0_CH0CONF:word32 and
     v1 = 0x00100000w:word32 and
     v2 = 0x00000000w:word32 in
-case dr.dr_xfer.state of
- | dr_xfer_not_ready => (NONE, NONE, dr)
- | dr_xfer_pre => (NONE, NONE, dr)
- | dr_xfer_idle => 
-   (SOME addr, SOME v1,
-    dr with dr_xfer := dr.dr_xfer with state := dr_xfer_conf_issued)
- | dr_xfer_conf_issued => (NONE, NONE, dr)
- | dr_xfer_read_txs => (NONE, NONE, dr)
- | dr_xfer_check_txs => (NONE, NONE, dr)
- | dr_xfer_write_dataO => (NONE, NONE, dr)
- | dr_xfer_read_rxs => (NONE, NONE, dr)
- | dr_xfer_check_rxs => (NONE, NONE, dr)
- | dr_xfer_read_rx0 => (NONE, NONE, dr)
- | dr_xfer_fetch_dataI => (NONE, NONE, dr)
- | dr_xfer_issue_disable => (NONE, NONE, dr)
- | dr_xfer_reset_conf => (SOME addr, SOME v2, 
-   dr with dr_xfer := dr.dr_xfer with state := dr_xfer_pre)`
+if (dr.state = dr_xfer_idle) then
+(SOME addr, SOME v1, dr with state := dr_xfer_conf_issued)
+else if (dr.state = dr_xfer_reset_conf) then
+(SOME addr, SOME v2, dr with state := dr_ready)
+else (NONE, NONE, dr with dr_err := T)`
 
 (* dr_write_ch0ctrl: driver_state -> word32 option * word32 option * driver_state *)
-(* TOFIX *)
 val dr_write_ch0ctrl_def = Define `
 dr_write_ch0ctrl (dr:driver_state) =
 let addr = SPI0_CH0CTRL:word32 and
     v1 = 0x00000001w:word32 and
     v2 = 0x00000000w:word32 in
-if (dr.dr_init.state = dr_init_done) /\ (dr.dr_tx.state = dr_tx_conf_issued) /\
-   (dr.dr_rx.state = dr_rx_idle) /\ (dr.dr_xfer.state = dr_xfer_idle) then
-   (SOME addr, SOME v1, 
-    dr with dr_tx := dr.dr_tx with state := dr_tx_read_txs)
-else if (dr.dr_init.state = dr_init_done) /\ (dr.dr_tx.state = dr_tx_issue_disable) /\
-   (dr.dr_rx.state = dr_rx_idle) /\ (dr.dr_xfer.state = dr_xfer_idle) then
-   (SOME addr, SOME v2, 
-    dr with dr_tx := dr.dr_tx with state := dr_tx_reset_conf)
-else if (dr.dr_init.state = dr_init_done) /\ (dr.dr_tx.state = dr_tx_idle) /\
-   (dr.dr_rx.state = dr_rx_conf_issued) /\ (dr.dr_xfer.state = dr_xfer_idle) then
-   (SOME addr, SOME v1,
-    dr with dr_rx := dr.dr_rx with state := dr_rx_read_rxs)
-else if (dr.dr_init.state = dr_init_done) /\ (dr.dr_tx.state = dr_tx_idle) /\
-   (dr.dr_rx.state = dr_rx_issue_disable) /\ (dr.dr_xfer.state = dr_xfer_idle) then
-   (SOME addr, SOME v2, 
-    dr with dr_rx := dr.dr_rx with state := dr_rx_reset_conf)
-else if (dr.dr_init.state = dr_init_done) /\ (dr.dr_tx.state = dr_tx_idle) /\
-   (dr.dr_rx.state = dr_rx_idle) /\ (dr.dr_xfer.state = dr_xfer_conf_issued) then
-   (SOME addr, SOME v1,
-    dr with dr_xfer := dr.dr_xfer with state := dr_xfer_read_txs)
-else if (dr.dr_init.state = dr_init_done) /\ (dr.dr_tx.state = dr_tx_idle) /\
-   (dr.dr_rx.state = dr_rx_idle) /\ (dr.dr_xfer.state = dr_xfer_issue_disable) then
-   (SOME addr, SOME v2,
-   dr with dr_xfer := dr.dr_xfer with state := dr_xfer_reset_conf)
-else (NONE, NONE, dr)`
+if (dr.state = dr_tx_conf_issued) then
+(SOME addr, SOME v1, dr with state := dr_tx_read_txs)
+else if (dr.state = dr_tx_issue_disable) then
+(SOME addr, SOME v2, dr with state := dr_tx_reset_conf)
+else if (dr.state = dr_rx_conf_issued) then 
+(SOME addr, SOME v1, dr with state := dr_rx_read_rxs)
+else if (dr.state = dr_rx_issue_disable) then 
+(SOME addr, SOME v2, dr with state := dr_rx_reset_conf)
+else if (dr.state = dr_xfer_conf_issued) then
+(SOME addr, SOME v1, dr with state := dr_xfer_read_txs)
+else if (dr.state = dr_xfer_issue_disable) then
+(SOME addr, SOME v2, dr with state := dr_xfer_reset_conf)
+else (NONE, NONE, dr with dr_err := T)`
 
 (* dr_write_tx0: driver_state -> word32 option * word32 option * driver_state *)
 val dr_write_tx0_def = Define `
 dr_write_tx0 (dr:driver_state) = 
-if (dr.dr_tx.state = dr_tx_write_data) /\ (dr.dr_init.state = dr_init_done) /\
-   (dr.dr_rx.state = dr_rx_idle) /\ (dr.dr_xfer.state = dr_xfer_idle) /\
-   (dr.dr_tx.tx_cur_length < ((LENGTH dr.dr_tx.data_buf) - 1))
-then (SOME SPI0_TX0, SOME (w2w (EL (dr.dr_tx.tx_cur_length) (dr.dr_tx.data_buf))),
-      dr with dr_tx := dr.dr_tx with 
-      <|state := dr_tx_read_txs;
-      tx_cur_length := dr.dr_tx.tx_cur_length + 1 |>)
-else if (dr.dr_tx.state = dr_tx_write_data) /\ (dr.dr_init.state = dr_init_done) /\
-   (dr.dr_rx.state = dr_rx_idle) /\ (dr.dr_xfer.state = dr_xfer_idle) /\
-   (dr.dr_tx.tx_cur_length = ((LENGTH dr.dr_tx.data_buf) - 1))
-then (SOME SPI0_TX0, SOME (w2w (EL (dr.dr_tx.tx_cur_length) (dr.dr_tx.data_buf))),
-     dr with dr_tx := dr.dr_tx with 
-     <|state := dr_tx_read_eot;
-      tx_cur_length := dr.dr_tx.tx_cur_length + 1 |>)
-else if (dr.dr_xfer.state = dr_xfer_write_dataO) /\ (dr.dr_init.state = dr_init_done) /\
-    (dr.dr_tx.state = dr_tx_idle) /\ (dr.dr_rx.state = dr_rx_idle) /\
-    (dr.dr_xfer.xfer_cur_length <= ((LENGTH dr.dr_xfer.xfer_dataOUT_buf) -1))
-then (SOME SPI0_TX0, SOME (w2w (EL (dr.dr_xfer.xfer_cur_length) (dr.dr_xfer.xfer_dataOUT_buf))),
-     dr with dr_xfer := dr.dr_xfer with
-     <|state := dr_xfer_read_rxs;
-     xfer_cur_length := dr.dr_xfer.xfer_cur_length + 1|>)
-else (NONE, NONE, dr)`
+if (dr.state = dr_tx_write_data) /\ 
+(dr.dr_tx.tx_cur_length < ((LENGTH dr.dr_tx.tx_data_buf) - 1)) then 
+(SOME SPI0_TX0, SOME (w2w (EL (dr.dr_tx.tx_cur_length) (dr.dr_tx.tx_data_buf))),
+dr with <| dr_tx := dr.dr_tx with tx_cur_length := dr.dr_tx.tx_cur_length + 1;
+state := dr_tx_read_txs |>)
+else if (dr.state = dr_tx_write_data) /\
+(dr.dr_tx.tx_cur_length = ((LENGTH dr.dr_tx.tx_data_buf) - 1)) then 
+(SOME SPI0_TX0, SOME (w2w (EL (dr.dr_tx.tx_cur_length) (dr.dr_tx.tx_data_buf))),
+dr with <| dr_tx := dr.dr_tx with tx_cur_length := dr.dr_tx.tx_cur_length + 1;
+state := dr_tx_read_eot |>)
+else if (dr.state = dr_xfer_write_dataO) then 
+(SOME SPI0_TX0, SOME (w2w (EL (dr.dr_xfer.xfer_cur_length) (dr.dr_xfer.xfer_dataOUT_buf))),
+dr with <| dr_xfer := dr.dr_xfer with xfer_cur_length := dr.dr_xfer.xfer_cur_length + 1;
+state := dr_xfer_read_rxs |>)
+else (NONE, NONE, dr with dr_err := T)`
 
-(* INIT_WR_ENABLE:driver_state -> bool
- * driver is eligible to issue write commands within init state.
- *)
-val INIT_WR_ENABLE_def = Define `
-INIT_WR_ENABLE (dr:driver_state) =
-(dr.dr_init.state = dr_init_idle \/ 
-dr.dr_init.state = dr_init_setting)`
-
-(* TX_WR_ENABLE:driver_state -> bool
- * driver is eligible to issue write commands within tx state.
- *)
-val TX_WR_ENABLE_def = Define `
-TX_WR_ENABLE (dr:driver_state) =
-(dr.dr_tx.state = dr_tx_idle \/
- dr.dr_tx.state = dr_tx_conf_issued \/ 
- dr.dr_tx.state = dr_tx_write_data \/
- dr.dr_tx.state = dr_tx_issue_disable \/ 
- dr_tx_issue_disable = dr_tx_reset_conf)`
-
-(* RX_WR_ENABLE:driver_state -> bool
- * driver is eligible to issue write commands within rx state.
- *)
-val RX_WR_ENABLE_def = Define `
-RX_WR_ENABLE (dr:driver_state) =
-(dr.dr_rx.state = dr_rx_idle \/
- dr.dr_rx.state = dr_rx_conf_issued \/ 
- dr.dr_rx.state = dr_rx_issue_disable \/
- dr.dr_rx.state = dr_rx_reset_conf)`
-
-(* XFER_WR_ENABLE:driver_state -> bool
- * driver is eligible to issue write commands within xfer state.
- *)
-val XFER_WR_ENABLE_def = Define `
-XFER_WR_ENABLE (dr:driver_state) =
-(dr.dr_xfer.state = dr_xfer_idle \/
- dr.dr_xfer.state = dr_xfer_conf_issued \/
- dr.dr_xfer.state = dr_xfer_write_dataO \/
- dr.dr_xfer.state = dr_xfer_issue_disable \/
- dr.dr_xfer.state = dr_xfer_reset_conf)`
-
-(* dr_write:driver_state -> word32 option * word32 option * word32 option *)
+(* dr_write: driver_state -> word32 option * word32 option * driver_state *)
 val dr_write_def = Define `
 dr_write (dr:driver_state) =
-if dr.dr_err then (NONE, NONE, dr)
-else if (INIT_WR_ENABLE dr) /\ (dr.dr_init.state = dr_init_idle \/ dr.dr_init.state = dr_init_done) 
-then (dr_write_softreset dr)
-else if (INIT_WR_ENABLE dr) /\ (dr.dr_init.state = dr_init_setting) /\ (~ dr.dr_init.issue_wr_sysconfig)
-then (dr_write_sysconfig dr)
-else if (INIT_WR_ENABLE dr) /\ (dr.dr_init.state = dr_init_setting) /\ (~ dr.dr_init.issue_wr_modulctrl)
-then (dr_write_modulctrl dr)
-else if (INIT_WR_ENABLE dr) /\ (dr.dr_init.state = dr_init_setting) /\ (~ dr.dr_init.issue_wr_ch0conf_wl)
-then (dr_write_ch0conf_wl dr)
-else if (INIT_WR_ENABLE dr) /\ (dr.dr_init.state = dr_init_setting) /\ (~ dr.dr_init.issue_wr_ch0conf_mode)
-then (dr_write_ch0conf_mode dr)
-else if (INIT_WR_ENABLE dr) /\ (dr.dr_init.state = dr_init_setting) /\ (~ dr.dr_init.issue_wr_ch0conf_speed)
-then (dr_write_ch0conf_speed dr)
-else if (TX_WR_ENABLE dr) /\ (dr.dr_tx.state = dr_tx_idle \/ dr.dr_tx.state = dr_tx_reset_conf)
-then (dr_write_ch0conf_tx dr)
-else if (TX_WR_ENABLE dr) /\ (dr.dr_tx.state = dr_tx_conf_issued \/ dr.dr_tx.state = dr_tx_issue_disable) 
-then (dr_write_ch0ctrl dr)
-else if (TX_WR_ENABLE dr) /\ (dr.dr_tx.state = dr_tx_write_data)
-then (dr_write_tx0 dr)
-else if (RX_WR_ENABLE dr) /\ (dr.dr_rx.state = dr_rx_idle \/ dr.dr_rx.state = dr_rx_reset_conf)
-then (dr_write_ch0conf_rx dr)
-else if (RX_WR_ENABLE dr) /\ (dr.dr_rx.state = dr_rx_conf_issued \/ dr.dr_rx.state = dr_rx_issue_disable)
-then (dr_write_ch0ctrl dr)
-else if (XFER_WR_ENABLE dr) /\ (dr.dr_xfer.state = dr_xfer_idle \/ dr.dr_xfer.state = dr_xfer_reset_conf)
-then (dr_write_ch0conf_xfer dr)
-else if (XFER_WR_ENABLE dr) /\ (dr.dr_xfer.state = dr_xfer_conf_issued \/ dr.dr_xfer.state = dr_xfer_issue_disable)
-then (dr_write_ch0ctrl dr)
-else if (XFER_WR_ENABLE dr) /\ (dr.dr_xfer.state = dr_xfer_write_dataO)
-then (dr_write_tx0 dr)
-(* other conditions, no write commands issued *)
-else (NONE, NONE, dr)`
+case dr.state of
+ | dr_init_pre => (NONE, NONE, dr with dr_err := T)
+ | dr_init_idle => (dr_write_softreset dr)
+ | dr_init_read_req => (NONE, NONE, dr with dr_err := T)
+ | dr_init_check_rep => (NONE, NONE, dr with dr_err := T)
+ | dr_init_setting => if (~ dr.dr_init.issue_wr_sysconfig) then (dr_write_sysconfig dr)
+   else if (~ dr.dr_init.issue_wr_modulctrl) then (dr_write_modulctrl dr)
+   else if (~ dr.dr_init.issue_wr_ch0conf_wl) then (dr_write_ch0conf_wl dr)
+   else if (~ dr.dr_init.issue_wr_ch0conf_mode) then (dr_write_ch0conf_mode dr)
+   else if (~ dr.dr_init.issue_wr_ch0conf_speed) then (dr_write_ch0conf_speed dr)
+   else (NONE, NONE, dr)
+ | dr_ready => (NONE, NONE, dr with dr_err := T)
+ | dr_tx_idle => (dr_write_ch0conf_tx dr)
+ | dr_tx_conf_issued => (dr_write_ch0ctrl dr)
+ | dr_tx_read_txs => (NONE, NONE, dr with dr_err := T)
+ | dr_tx_check_txs => (NONE, NONE, dr with dr_err := T)
+ | dr_tx_write_data => (dr_write_tx0 dr)
+ | dr_tx_read_eot => (NONE, NONE, dr with dr_err := T)
+ | dr_tx_check_eot => (NONE,NONE, dr with dr_err := T)
+ | dr_tx_issue_disable => (dr_write_ch0ctrl dr)
+ | dr_tx_reset_conf => (dr_write_ch0conf_tx dr)
+ | dr_rx_idle => (dr_write_ch0conf_rx dr)
+ | dr_rx_conf_issued => (dr_write_ch0ctrl dr)
+ | dr_rx_read_rxs => (NONE, NONE, dr with dr_err := T)
+ | dr_rx_check_rxs => (NONE, NONE, dr with dr_err := T)
+ | dr_rx_read_rx0 => (NONE, NONE, dr with dr_err := T)
+ | dr_rx_fetch_data => (NONE, NONE, dr with dr_err := T)
+ | dr_rx_issue_disable => (dr_write_ch0ctrl dr)
+ | dr_rx_reset_conf => (dr_write_ch0conf_rx dr)
+ | dr_xfer_idle => (dr_write_ch0conf_xfer dr)
+ | dr_xfer_conf_issued => (dr_write_ch0ctrl dr)
+ | dr_xfer_read_txs => (NONE, NONE, dr with dr_err := T)
+ | dr_xfer_check_txs => (NONE, NONE, dr with dr_err := T)
+ | dr_xfer_write_dataO => (dr_write_tx0 dr)
+ | dr_xfer_read_rxs => (NONE, NONE, dr with dr_err := T)
+ | dr_xfer_check_rxs => (NONE, NONE, dr with dr_err := T)
+ | dr_xfer_read_rx0 => (NONE, NONE, dr with dr_err := T)
+ | dr_xfer_fetch_dataI => (NONE, NONE, dr with dr_err := T)
+ | dr_xfer_issue_disable => (dr_write_ch0ctrl dr)
+ | dr_xfer_reset_conf => (dr_write_ch0conf_xfer dr)`
+
+(* dr_write_address: driver_state -> word32 option *)
+val dr_write_address_def = Define `
+dr_write_address (dr:driver_state) =
+let (ad, v, dr') = dr_write dr in ad`
+
+(* dr_write_value: driver_state -> word32 option *)
+val dr_write_value_def = Define `
+dr_write_value (dr:driver_state) =
+let (ad, v, dr') = dr_write dr in v`
+
+(* dr_write_state: driver_state -> driver_state *)
+val dr_write_state_def = Define `
+dr_write_state (dr:driver_state) =
+let (ad, v, dr') = dr_write dr in dr'`
 
 val _ = export_theory();
