ds_abs1/ds_abs1_initScript.sml
@@ -1,83 +1,29 @@
 open HolKernel bossLib boolLib Parse;
-open ds_abs1_stateTheory board_memTheory;
+open ds_abs1_stateTheory;
 
 val _ = new_theory "ds_abs1_init";
-
-(* COMB_ABS1_INIT_ENABLE: ds_abs1_state -> bool *)
-val COMB_ABS1_INIT_ENABLE_def = Define `
-COMB_ABS1_INIT_ENABLE (ds_abs1:ds_abs1_state) =
-((ds_abs1.ds_abs1_init.state = abs1_init_start) \/
-(ds_abs1.ds_abs1_init.state = abs1_init_done))`
-
-
-(* spi_abs1_init_start_op: ds_abs1_state -> ds_abs1_state 
-val spi_abs1_init_start_op_def = Define `
-spi_abs1_init_start_op (ds_abs1:ds_abs1_state) =
-ds_abs1 with 
-ds_abs1_init := ds_abs1.ds_abs1_init with state := abs1_init_check`
-
-
-(* spi_abs1_init_operations: ds_abs1_state -> ds_abs1_state *)
-val spi_abs1_init_operations_def = Define `
-spi_abs1_init_operations (ds_abs1:ds_abs1_state) = 
-if ds_abs1.ds_abs1_init.state = abs1_init_start then spi_abs1_init_start_op ds_abs1
-else ds_abs1 with err := T`
-
-(* driver_abs1_init_start_op: ds_abs1_state -> ds_abs1_state *)
-val driver_abs1_init_start_op_def = Define `
-driver_abs1_init_start_op (ds_abs1:ds_abs1_state) =
-ds_abs1 with driver_abs1 := ds_abs1.driver_abs1 with 
-<| dr_abs1_last_read_ad := (SOME SPI0_SYSSTATUS); dr_abs1_last_read_v := (SOME 0w) |>`
-
-(* driver_abs1_init_check_op: ds_abs1_state -> ds_abs1_state *)
-val driver_abs1_init_check_op_def = Define `
-driver_abs1_init_check_op (ds_abs1:ds_abs1_state) =
-if (ds_abs1.driver_abs1.dr_abs1_last_read_ad = (SOME SPI0_SYSSTATUS)) /\
-   (ds_abs1.driver_abs1.dr_abs1_last_read_v = (SOME 0w)) 
-then ds_abs1 with driver_abs1 := ds_abs1.driver_abs1 with 
-     dr_abs1_last_read_v := (SOME 1w)
-else ds_abs1 with 
-<| ds_abs1_init := ds_abs1.ds_abs1_init with state := abs1_init_done;
-driver_abs1 := ds_abs1.driver_abs1 with 
-<| dr_abs1_last_read_ad := (SOME SPI0_SYSSTATUS); dr_abs1_last_read_v := (SOME 1w) |> |>`
-
-(* driver_abs1_init_operations: ds_abs1_state -> ds_abs1_state *)
-val driver_abs1_init_operations_def = Define `
-driver_abs1_init_operations (ds_abs1:ds_abs1_state) = 
-case ds_abs1.ds_abs1_init.state of
-  | abs1_init_start => driver_abs1_init_start_op ds_abs1
-  | abs1_init_check => driver_abs1_init_check_op ds_abs1
-  | abs1_init_done => ds_abs1 with err := T`
-*)
-
-(* comb_abs1_init_start_op: ds_abs1_state -> ds_abs1_state *)
-val comb_abs1_init_start_op_def = Define `
-comb_abs1_init_start_op (ds_abs1: ds_abs1_state) =
-ds_abs1 with <|
-ds_abs1_init := ds_abs1.ds_abs1_init with state := abs1_init_done;
-ds_abs1_tx := ds_abs1.ds_abs1_tx with state := abs1_tx_pre;
-ds_abs1_rx := ds_abs1.ds_abs1_rx with state := abs1_rx_pre;
-ds_abs1_xfer := ds_abs1.ds_abs1_xfer with state := abs1_xfer_pre |>`
-
-
-(* comb_abs1_init_done_op: ds_abs1_state -> ds_abs1_state *)
-val comb_abs1_init_done_op_def = Define `
-comb_abs1_init_done_op (ds_abs1: ds_abs1_state) =
-ds_abs1 with ds_abs1_init := ds_abs1.ds_abs1_init with state := abs1_init_start`
-
-
-(* comb_abs1_init_operations: ds_abs1_state -> ds_abs1_state *)
-val comb_abs1_init_operations_def = Define `
-comb_abs1_init_operations (ds_abs1:ds_abs1_state) = 
-case ds_abs1.ds_abs1_init.state of
-  | abs1_init_pre => ds_abs1 with err := T
-  | abs1_init_start => comb_abs1_init_start_op ds_abs1
-  | abs1_init_done => comb_abs1_init_done_op ds_abs1`
 
 (* call_init_ds_abs1:ds_abs1_state -> ds_abs1_state *)
 val call_init_ds_abs1_def = Define `
 call_init_ds_abs1 (ds_abs1:ds_abs1_state) =
-ds_abs1 with ds_abs1_init := ds_abs1.ds_abs1_init with 
-state := abs1_init_start`
+ds_abs1 with state := abs1_init_start`
+
+(* COMB_ABS1_INIT_ENABLE: ds_abs1_state -> bool *)
+val COMB_ABS1_INIT_ENABLE_def = Define `
+COMB_ABS1_INIT_ENABLE (ds_abs1:ds_abs1_state) =
+(ds_abs1.state = abs1_init_start)`
+
+(* comb_abs1_init_start_op: ds_abs1_state -> ds_abs1_state *)
+val comb_abs1_init_start_op_def = Define `
+comb_abs1_init_start_op (ds_abs1: ds_abs1_state) =
+ds_abs1 with state := abs1_ready`
+
+(* comb_abs1_init_operations: ds_abs1_state -> ds_abs1_state *)
+val comb_abs1_init_operations_def = Define `
+comb_abs1_init_operations (ds_abs1:ds_abs1_state) = 
+if (ds_abs1.state = abs1_init_start) then
+(comb_abs1_init_start_op ds_abs1)
+else ds_abs1 with err := T`
+
 
 val _ = export_theory();
