ds_abs1/ds_abs1_relScript.sml
@@ -4,11 +4,8 @@ open ds_abs1_stateTheory ds_abs1_initTheory ds_abs1_txTheory ds_abs1_rxTheory ds
 
 val _ = new_theory "ds_abs1_rel"
 
-
-(* ds_abs1_spi_tr: spi abstract level1 model transtion *)
+(* ds_abs1_spi_tr: spi abstract model transtion *)
 val (ds_abs1_spi_tr_rules, ds_abs1_spi_tr_ind, ds_abs1_spi_tr_cases) = Hol_reln `
-(* (!(ds_abs1:ds_abs1_state). (SPI_ABS1_INIT_ENABLE ds_abs1) ==>
-ds_abs1_spi_tr ds_abs1 tau_spi (spi_abs1_init_operations ds_abs1)) /\ *)
 (!(ds_abs1:ds_abs1_state). (SPI_ABS1_TX_ENABLE ds_abs1) ==>
 ds_abs1_spi_tr ds_abs1 tau_spi (spi_abs1_tx_operations ds_abs1)) /\
 (!(ds_abs1:ds_abs1_state). (SPI_ABS1_RX_ENABLE ds_abs1) ==>
@@ -17,19 +14,15 @@ ds_abs1_spi_tr ds_abs1 tau_spi (spi_abs1_rx_operations ds_abs1)) /\
 ds_abs1_spi_tr ds_abs1 tau_spi (spi_abs1_xfer_operations ds_abs1))`
 
 
-(* ds_abs1_dr_tr: driver abstract level1 model transtion *)
+(* ds_abs1_dr_tr: driver abstract model transtion *)
 val (ds_abs1_dr_tr_rules, ds_abs1_dr_tr_ind, ds_abs1_dr_tr_cases) = Hol_reln `
-(* (!(ds_abs1:ds_abs1_state). (DRIVER_ABS1_INIT_ENABLE ds_abs1) ==>
-ds_abs1_dr_tr ds_abs1 tau_dr (driver_abs1_init_operations ds_abs1)) /\ *)
-(!(ds_abs1:ds_abs1_state). (DRIVER_ABS1_TX_ENABLE ds_abs1) ==>
-ds_abs1_dr_tr ds_abs1 tau_dr (driver_abs1_tx_operations ds_abs1)) /\
 (!(ds_abs1:ds_abs1_state). (DRIVER_ABS1_RX_ENABLE ds_abs1) ==>
 ds_abs1_dr_tr ds_abs1 tau_dr (driver_abs1_rx_operations ds_abs1)) /\
 (!(ds_abs1:ds_abs1_state). (DRIVER_ABS1_XFER_ENABLE ds_abs1) ==>
 ds_abs1_dr_tr ds_abs1 tau_dr (driver_abs1_xfer_operations ds_abs1))`
 
 
-(* ds_abs1_comb_tr: the combined level1 model transtion *)
+(* ds_abs1_comb_tr: the combined model transtion *)
 val (ds_abs1_comb_tr_rules, ds_abs1_comb_tr_ind, ds_abs1_comb_tr_cases) = Hol_reln `
 (!(ds_abs1:ds_abs1_state). (COMB_ABS1_INIT_ENABLE ds_abs1) ==>
 ds_abs1_comb_tr ds_abs1 tau_comb (comb_abs1_init_operations ds_abs1)) /\
@@ -41,28 +34,31 @@ ds_abs1_comb_tr ds_abs1 tau_comb (comb_abs1_rx_operations ds_abs1)) /\
 ds_abs1_comb_tr ds_abs1 tau_comb (comb_abs1_xfer_operations ds_abs1))`
 
 
-(* ds_abs1_tr: the combined abstract level1 model transtion *)
+(* ds_abs1_tr: the combined abstract state transtion *)
 val (ds_abs1_tr_rules, ds_abs1_tr_ind, ds_abs1_tr_cases) = Hol_reln `
-(!(ds_abs1:ds_abs1_state). ds_abs1.ds_abs1_init.state = abs1_init_pre ==>
+(* interface for other programs to call the abstract model functions *)
+(!(ds_abs1:ds_abs1_state). (ds_abs1.state = abs1_init_pre) \/ (ds_abs1.state = abs1_ready) ==>
 ds_abs1_tr ds_abs1 call_init (call_init_ds_abs1 ds_abs1)) /\
-(!(ds_abs1:ds_abs1_state). (ds_abs1.ds_abs1_tx.state = abs1_tx_pre) /\ (buffer <> []) ==>
+(!(ds_abs1:ds_abs1_state). (ds_abs1.state = abs1_ready) /\ (buffer <> []) ==>
 ds_abs1_tr ds_abs1 (call_tx buffer) (call_tx_ds_abs1 ds_abs1 buffer)) /\
-(!(ds_abs1:ds_abs1_state). (ds_abs1.ds_abs1_rx.state = abs1_rx_pre) /\ (length > 0) ==>
+(!(ds_abs1:ds_abs1_state). (ds_abs1.state = abs1_ready) /\ (length > 0) ==>
 ds_abs1_tr ds_abs1 (call_rx length) (call_rx_ds_abs1 ds_abs1 length)) /\
-(!(ds_abs1:ds_abs1_state). (ds_abs1.ds_abs1_xfer.state = abs1_xfer_pre) /\ (buffer <> []) ==>
+(!(ds_abs1:ds_abs1_state). (ds_abs1.state = abs1_ready) /\ (buffer <> []) ==>
 ds_abs1_tr ds_abs1 (call_xfer buffer) (call_xfer_ds_abs1 ds_abs1 buffer)) /\
+(* tau transition in the model *)
 (!(ds_abs1:ds_abs1_state). ds_abs1_spi_tr ds_abs1 tau_spi ds_abs1' ==>
 ds_abs1_tr ds_abs1 tau ds_abs1') /\
 (!(ds_abs1:ds_abs1_state). ds_abs1_dr_tr ds_abs1 tau_dr ds_abs1' ==>
 ds_abs1_tr ds_abs1 tau ds_abs1') /\
 (!(ds_abs1:ds_abs1_state). ds_abs1_comb_tr ds_abs1 tau_comb ds_abs1' ==>
 ds_abs1_tr ds_abs1 tau ds_abs1') /\
+(* cases for the model to transfer data with another spi device *)
 (!(ds_abs1:ds_abs1_state). (ABS1_TX_LBL_ENABLE ds_abs1) ==>
 ds_abs1_tr ds_abs1 (TX (abs1_tx_trans_done_op_value ds_abs1)) 
 (abs1_tx_trans_done_op_state ds_abs1)) /\
-(!(ds_abs1:ds_abs1_state). (ABS1_RX_LBL_ENABLE ds_abs1) ==>
+(!(ds_abs1:ds_abs1_state). (ABS1_RX_LBL_ENABLE ds_abs1) /\ (data <> NONE) ==>
 ds_abs1_tr ds_abs1 (RX data) (abs1_rx_receive_data_op ds_abs1 data)) /\
-(!(ds_abs1:ds_abs1_state). (ds_abs1.ds_abs1_xfer.state = abs1_xfer_exchange) ==>
+(!(ds_abs1:ds_abs1_state). (ds_abs1.state = abs1_xfer_exchange) /\ (dataIN <> NONE) ==>
 ds_abs1_tr ds_abs1 (XFER dataIN (abs1_xfer_exchange_op_value ds_abs1 dataIN)) 
 (abs1_xfer_exchange_op_state ds_abs1 dataIN))`
 
