ds_abs1/ds_abs1_stateScript.sml
@@ -2,55 +2,37 @@ open HolKernel bossLib boolLib Parse;
 open wordsLib wordsTheory;
 open SPI_stateTheory driver_stateTheory;
 
-(* ds_abs1: driver and spi controller combined abstract model (level1) states.
+(* ds_abs1: SPI driver and controller combined abstract model states.
  * This abstract model removes the interactions of the driver and spi controller, 
- * including Write/Update, Read/Return.
- * We assume that the driver model commands are correct considering the spi model.
+ * including Write/Update, Read/Return, and some spi and driver tau transitions.
  *)
 val _ = new_theory "ds_abs1_state";
 
-(* ds_abs1_init_state: the state of ds_abs1 init automaton *)
-val _ = Datatype `ds_abs1_init_general_state =
-| abs1_init_pre | abs1_init_start | abs1_init_done`
-
-val _ = Datatype `ds_abs1_init_state = <|
-state : ds_abs1_init_general_state |>`
+(* ds_abs1_general_state: the general states of ds_abs1 model *)
+val _ = Datatype `ds_abs1_general_state =
+| abs1_init_pre | abs1_init_start | abs1_ready
+| abs1_tx_idle | abs1_tx_trans | abs1_tx_data_1 | abs1_tx_data_2
+| abs1_tx_done_1 | abs1_tx_done_2 | abs1_tx_reset
+| abs1_rx_idle | abs1_rx_receive | abs1_rx_update | abs1_rx_ready
+| abs1_rx_fetch_data | abs1_rx_done | abs1_rx_next 
+| abs1_rx_next_ready | abs1_rx_stop | abs1_rx_reset
+| abs1_xfer_idle | abs1_xfer_prepare | abs1_xfer_trans
+| abs1_xfer_data | abs1_xfer_exchange | abs1_xfer_update
+| abs1_xfer_ready | abs1_xfer_fetch_data | abs1_xfer_reset`
 
 (* ds_abs1_tx_state: the state of ds_abs1 tx automaton *)
-val _ = Datatype `ds_abs1_tx_general_state =
-| abs1_tx_not_ready | abs1_tx_pre | abs1_tx_idle | abs1_tx_prepare 
-| abs1_tx_trans | abs1_tx_data_1 | abs1_tx_data_2
-| abs1_tx_done_1 | abs1_tx_done_2 | abs1_tx_done_3
-| abs1_tx_check_1 | abs1_tx_check_2 | abs1_tx_check_3 
-| abs1_tx_next | abs1_tx_ready_for_reset | abs1_tx_reset`
-
 val _ = Datatype `ds_abs1_tx_state = <|
-state: ds_abs1_tx_general_state;
 tx_data_buffer: word8 list;
 tx_cur_length: num |>`
 
 (* ds_abs1_rx_state: the state of ds_abs1 rx automaton *)
-val _ = Datatype `ds_abs1_rx_general_state =
-| abs1_rx_not_ready | abs1_rx_pre | abs1_rx_idle | abs1_rx_receive 
-| abs1_rx_update | abs1_rx_ready | abs1_rx_fetch_data 
-| abs1_rx_return | abs1_rx_done | abs1_rx_last 
-| abs1_rx_check_1 | abs1_rx_check_2 | abs1_rx_pre_reset 
-| abs1_rx_ready_for_reset | abs1_rx_reset`
-
 val _ = Datatype `ds_abs1_rx_state = <|
-state: ds_abs1_rx_general_state;
 rx_data_buffer: word8 list;
-rx_left_length: num |>`
+rx_left_length: num;
+temp_value: word8 |>`
 
 (* ds_abs1_xfer_state: the state of ds_abs1 xfer automaton *)
-val _ = Datatype `ds_abs1_xfer_general_state =
-| abs1_xfer_not_ready | abs1_xfer_pre | abs1_xfer_idle | abs1_xfer_prepare 
-| abs1_xfer_trans | abs1_xfer_data | abs1_xfer_exchange | abs1_xfer_update 
-| abs1_xfer_ready | abs1_xfer_fetch_data | abs1_xfer_next | abs1_xfer_next_write 
-| abs1_xfer_done | abs1_xfer_ready_for_reset | abs1_xfer_reset`
-
 val _ = Datatype `ds_abs1_xfer_state = <|
-state: ds_abs1_xfer_general_state;
 xfer_dataIN_buffer: word8 list;
 xfer_dataOUT_buffer: word8 list;
 xfer_cur_length: num |>`
@@ -59,18 +41,11 @@ val _ = Datatype `spi_abs1_state = <|
 TX_SHIFT_REG: word8;
 RX_SHIFT_REG: word8 |>`
 
-(* only used for internal states transition 
-val _ = Datatype `driver_abs1_state = <|
-dr_abs1_last_read_ad: word32 option;
-dr_abs1_last_read_v: word32 option |>`
-*)
-
 (* ds_abs1_state: the state of the spi controller and driver combined abstract level1 model *)
 val _ = Datatype `ds_abs1_state = <|
 err: bool;
+state: ds_abs1_general_state;
 spi_abs1: spi_abs1_state;
-(* driver_abs1: driver_abs1_state;  TO REMOVE*)
-ds_abs1_init: ds_abs1_init_state;
 ds_abs1_tx: ds_abs1_tx_state;
 ds_abs1_rx: ds_abs1_rx_state;
 ds_abs1_xfer: ds_abs1_xfer_state |>`
