spi_model/SPI_data_trScript.sml
@@ -1,0 +1,59 @@
+open HolKernel bossLib boolLib Parse;
+open wordsTheory wordsLib;
+open SPI_stateTheory board_memTheory;
+
+val _ = new_theory "SPI_data_tr";
+
+(* SPI data transition for TX label *)
+(* This function returns a new spi state and the data to be transmitted.
+ * tx_trans_done_op: spi_state -> spi_state * word8 option
+ *)
+val tx_trans_done_op_def = Define `
+tx_trans_done_op (spi:spi_state) = 
+(spi with <|regs := spi.regs with CH0STAT := spi.regs.CH0STAT
+(* An SPI word is transferred from the TX shift register to the slave *)
+with EOT := 1w;
+state := tx_ready_for_trans |>,
+SOME spi.TX_SHIFT_REG)`
+
+(* return specific datatype from above function *)
+val tx_trans_done_op_state_def = Define `
+tx_trans_done_op_state (spi:spi_state) =
+let (spi', v_option) = tx_trans_done_op spi in spi'`
+
+val tx_trans_done_op_value_def = Define `
+tx_trans_done_op_value (spi:spi_state) =
+let (spi', v_option) = tx_trans_done_op spi in v_option`
+
+(* SPI data transition for RX label *)
+(* rx_receive_data_op: spi_state -> word8 option -> spi_state *)
+val rx_receive_data_op_def = Define `
+rx_receive_data_op (spi:spi_state) (data:word8 option) =
+if (data <> NONE) then 
+spi with <| RX_SHIFT_REG := THE data; (* a word is received over the wire *)
+state := rx_update_RX0 |>
+else spi with err := T`
+
+(* SPI data transition for XFER label *)
+(* Master TX_shift_reg -> Slave RX_shift_reg and Slave TX_shift_reg -> Master RX_Shift_reg.
+ * xfer_exchange_data_op_def: spi_state -> word8 option-> spi_state * word8 option
+ *)
+val xfer_exchange_data_op_def = Define `
+xfer_exchange_data_op (spi:spi_state) (dataIN:word8 option) =
+if (dataIN <> NONE) then
+(spi with <|regs := spi.regs with CH0STAT := spi.regs.CH0STAT with EOT := 1w;
+RX_SHIFT_REG := (THE dataIN);
+state := xfer_update_RX0 |>,
+SOME spi.TX_SHIFT_REG)
+else (spi with err := T, NONE)`
+
+(* return specific datatype from above function *)
+val xfer_exchange_data_op_state_def = Define `
+xfer_exchange_data_op_state (spi:spi_state) (dataIN: word8 option) =
+let (spi', v_option) = xfer_exchange_data_op spi dataIN in spi'`
+
+val xfer_exchange_data_op_value_def = Define `
+xfer_exchange_data_op_value (spi:spi_state) (dataIN: word8 option) =
+let (spi', v_option) = xfer_exchange_data_op spi dataIN in v_option`
+
+val _ = export_theory();
