spi_model/SPI_tauScript.sml
@@ -1,0 +1,134 @@
+open HolKernel bossLib boolLib Parse;
+open wordsTheory wordsLib;
+open SPI_stateTheory board_memTheory;
+
+val _ = new_theory "SPI_tau";
+
+(* SPI is in a state to perform tau transition.
+ * SPI_TAU_ENABLE: spi_state -> bool *)
+val SPI_TAU_ENABLE_def = Define `
+SPI_TAU_ENABLE (spi:spi_state) =
+((spi.state = init_reset) \/ (spi.state = tx_channel_enabled) \/
+(spi.state = tx_trans_data) \/ (spi.state = rx_channel_enabled) \/
+(spi.state = rx_update_RX0) \/ (spi.state = xfer_channel_enabled) \/
+(spi.state = xfer_trans_data) \/ (spi.state = xfer_update_RX0))`
+
+
+(* internal operations for init automaton *)
+(* SPI controller performs reset operation.
+ * init_reset_op: spi_state -> spi_state
+ *)
+val init_reset_op_def = Define `
+init_reset_op (spi:spi_state) = 
+spi with <| regs := spi.regs with SYSSTATUS := 1w (* indiciate reset is done *);
+state := init_setregs (* enter the next init state, set up SPI registers *) |>`
+
+
+(* internal operations for tx automaton *)
+(* SPI controller operations when channel 0 is enabled for tx.
+ * tx_channel_enabled_op: spi_state -> spi_state
+ *)
+val tx_channel_enabled_op_def = Define `
+tx_channel_enabled_op (spi:spi_state) =
+spi with <|regs := spi.regs with CH0STAT := spi.regs.CH0STAT 
+with <|TXS := 1w; EOT := 0w |>;
+state := tx_ready_for_trans |>`
+
+(* SPI controller's operation after TX0 register was set. 
+ * TX0 -> TX_SHIFT_REG, SPI internal data transition.
+ * tx_trans_data_op: spi_state -> spi_state 
+ *)
+val tx_trans_data_op_def = Define `
+tx_trans_data_op (spi:spi_state) =
+spi with <| TX_SHIFT_REG := w2w spi.regs.TX0;
+regs := spi.regs with CH0STAT := spi.regs.CH0STAT
+with <|EOT := 0w; TXS := 1w|>; (* cleat EOT bit, set TXS *)  
+state := tx_trans_done |>`
+
+(* internal operations for rx automaton *)
+(* SPI controller operation for rx mode when channel 0 is enabled.
+ * rx_channel_enabled_op : spi_state -> spi_state
+ *)
+val rx_channel_enabled_op_def = Define `
+rx_channel_enabled_op (spi:spi_state) =
+spi with <| regs := spi.regs with CH0STAT := spi.regs.CH0STAT
+with RXS := 0w (* RXS is cleared when enable the channel *);
+state := rx_receive_data |>`
+
+(* SPI uploads the data from the shift register to its RX0 register, RX_SHIFT_REG -> RX0.
+ * rx_update_RX0_op: spi_state -> spi_state
+ *)
+val rx_update_RX0_op_def = Define `
+rx_update_RX0_op (spi:spi_state) =
+spi with <| regs := spi.regs with
+(* a received word is transferred from shift register to RX0 *)
+<| RX0 := w2w spi.RX_SHIFT_REG;
+CH0STAT := spi.regs.CH0STAT with RXS := 1w |>;
+state := rx_data_ready |>`
+
+
+(* internal operations for xfer automaton *)
+(* SPI controller operations when channel 0 is enabled for xfer.
+ * xfer_channel_enabled_op:spi_state -> spi_state
+ *)
+val xfer_channel_enabled_op_def = Define `
+xfer_channel_enabled_op (spi:spi_state) = 
+spi with <| regs := spi.regs with CH0STAT := spi.regs.CH0STAT
+with <|RXS := 0w; TXS := 1w; EOT := 1w |>;
+state := xfer_ready_for_trans |>`
+
+(* Update theTX_SHIFT_REG after TX0 was written.
+ * TX0 -> SPI TX_SHIFT_REG
+ * xfer_trans_data_op : spi_state -> spi_state
+ *)
+val xfer_trans_data_op_def = Define `
+xfer_trans_data_op (spi:spi_state) =
+spi with <| (* TX0 -> TX_shift_register *)
+TX_SHIFT_REG := w2w spi.regs.TX0;
+regs := spi.regs with CH0STAT := spi.regs.CH0STAT
+with <| EOT := 0w; TXS := 1w |>;
+state := xfer_exchange_data |>`
+
+(* SPI controller handles the received word from shift register to RX0 
+ * xfer_update_RX0_op: spi_state -> spi_state
+ *)
+val xfer_update_RX0_op_def = Define `
+xfer_update_RX0_op (spi:spi_state) =
+spi with <| regs := spi.regs with
+(* shift register -> RX0 *)
+<| RX0 := w2w spi.RX_SHIFT_REG;
+CH0STAT := spi.regs.CH0STAT with RXS := 1w |>;
+state := xfer_data_ready |>`
+
+(* This function shows internal operations of SPI controller, spi tau spi'.
+ * spi_tau_operations: spi_state -> spi_state
+ *)
+val spi_tau_operations_def = Define `
+spi_tau_operations (spi:spi_state) =
+case spi.state of
+  | init_start => spi with err := T
+  | init_reset => init_reset_op spi
+  | init_setregs => spi with err := T
+  | spi_ready => spi with err := T
+  | tx_conf_ready => spi with err := T
+  | tx_channel_enabled => tx_channel_enabled_op spi
+  | tx_ready_for_trans => spi with err := T
+  | tx_trans_data => tx_trans_data_op spi
+  | tx_trans_done => spi with err := T
+  | tx_channel_disabled => spi with err := T
+  | rx_conf_ready => spi with err := T
+  | rx_channel_enabled => rx_channel_enabled_op spi
+  | rx_receive_data => spi with err := T
+  | rx_update_RX0 => rx_update_RX0_op spi
+  | rx_data_ready => spi with err := T
+  | rx_channel_disabled => spi with err := T
+  | xfer_conf_ready => spi with err := T
+  | xfer_channel_enabled => xfer_channel_enabled_op spi
+  | xfer_ready_for_trans => spi with err := T
+  | xfer_trans_data => xfer_trans_data_op spi
+  | xfer_exchange_data => spi with err := T
+  | xfer_update_RX0 => xfer_update_RX0_op spi
+  | xfer_data_ready => spi with err := T
+  | xfer_channel_disabled => spi with err :=T`
+
+val _ = export_theory();
