thm/abs1_comb_hold_ref_rel_dr_trScript.sml
@@ -9,6 +9,51 @@ open ref_relTheory;
 
 val _ = new_theory "abs1_comb_hold_ref_rel_spi_tr";
 
+val ref_rel_check_SYSSTATUS = store_thm("ref_rel_check_SYSSTATUS",
+``!(spi:spi_state) (dr:driver_state) (ds_abs1:ds_abs1_state).
+(ref_rel ds_abs1 dr spi) /\ (dr.dr_last_read_ad = SOME SPI0_SYSSTATUS) /\
+(dr.dr_last_read_v = SOME v) /\ (INIT_CHECK_ENABLE dr) ==>
+ref_rel ds_abs1 (dr_check_sysstatus dr v) spi``,
+rw [dr_check_sysstatus_def, INIT_CHECK_ENABLE_def] >|
+[FULL_SIMP_TAC std_ss [ref_rel_def] >>
+rw [] >>
+FULL_SIMP_TAC std_ss [IS_INIT_REL_def, IS_TX_REL_def, IS_RX_REL_def, IS_XFER_REL_def] >>
+rw [] >>
+Cases_on `spi.init.state` >>
+rw [] >>
+FULL_SIMP_TAC (std_ss++WORD_ss) [],
+FULL_SIMP_TAC std_ss [ref_rel_def] >>
+rw [] >>
+FULL_SIMP_TAC std_ss [IS_INIT_REL_def, IS_TX_REL_def, IS_RX_REL_def, IS_XFER_REL_def] >>
+rw []]);
+
+val ref_rel_check_CH0STAT_TX = store_thm("ref_rel_check_CH0STAT_TX",
+``!(spi:spi_state) (dr:driver_state) (ds_abs1:ds_abs1_state).
+(ref_rel ds_abs1 dr spi) /\ (dr.dr_last_read_ad = SOME SPI0_CH0STAT) /\
+(dr.dr_last_read_v = SOME v) /\ (TX_CHECK_ENABLE dr) ==>
+(ref_rel ds_abs1 (dr_check_ch0stat dr v) spi)``,
+rw [TX_CHECK_ENABLE_def, dr_check_ch0stat_def] >|
+[rw [dr_check_tx_ch0stat_def] >|
+[FULL_SIMP_TAC std_ss [ref_rel_def] >>
+rw [] >>
+FULL_SIMP_TAC std_ss [IS_INIT_REL_def, IS_TX_REL_def, IS_RX_REL_def, IS_XFER_REL_def] >>
+rw [] >>
+cheat,
+FULL_SIMP_TAC std_ss [ref_rel_def] >>
+rw [] >>
+FULL_SIMP_TAC std_ss [IS_INIT_REL_def, IS_TX_REL_def, IS_RX_REL_def, IS_XFER_REL_def] >>
+rw []],
+
+rw [dr_check_tx_ch0stat_def] >|
+[FULL_SIMP_TAC std_ss [ref_rel_def] >>
+rw [] >>
+FULL_SIMP_TAC std_ss [IS_INIT_REL_def, IS_TX_REL_def, IS_RX_REL_def, IS_XFER_REL_def] >>
+rw [] >>
+cheat,
+FULL_SIMP_TAC std_ss [ref_rel_def] >>
+rw [] >>
+FULL_SIMP_TAC std_ss [IS_INIT_REL_def, IS_TX_REL_def, IS_RX_REL_def, IS_XFER_REL_def] >>
+rw []]]);
 
 (* bi-simulation: ds_abs1' exists and holds the ref_rel when driver_tau *)
 val abs1_comb_hold_ref_rel_driver_tr = store_thm("abs1_comb_hold_ref_rel_driver_tr",
@@ -16,9 +61,21 @@ val abs1_comb_hold_ref_rel_driver_tr = store_thm("abs1_comb_hold_ref_rel_driver_
 (ref_rel ds_abs1 dr spi) /\ (driver_tr dr tau dr') ==>
 (ref_rel ds_abs1 dr' spi) \/
 (?ds_abs1'. (ds_abs1_tr ds_abs1 tau ds_abs1') /\ (ref_rel ds_abs1' dr' spi))``,
-rw [driver_tr_cases, dr_check_def] >>
-rw [dr_check_sysstatus_def] >>
-cheat);
+rw [driver_tr_cases] >|
+[
+FULL_SIMP_TAC std_ss [dr_tx_syn_tr_cases] >>
+rw [] >>
+cheat,
+cheat,
+cheat,
+
+rw [dr_check_def] >>
+rw [ref_rel_check_SYSSTATUS]
+rw [ref_rel_check_CH0STAT_TX]
+rw [ref_rel_check_CH0STAT_RX]
+
+
+]);
 
 
 val _ = export_theory();
