thm/ref_rel_holds_trans_lblScript.sml
@@ -1,46 +1,47 @@
 open HolKernel bossLib boolLib Parse;
-open SPI_stateTheory SPI_relationTheory SPI_txTheory SPI_rxTheory SPI_xferTheory;
+open SPI_stateTheory SPI_relationTheory SPI_data_trTheory;
 open driver_stateTheory driver_relationTheory;
 open ds_abs1_stateTheory ds_abs1_relTheory ds_abs1_txTheory ds_abs1_rxTheory ds_abs1_xferTheory;
 open ref_relTheory;
 
 val _ = new_theory "ref_rel_holds_trans_lbl";
 
-(* a help lemma to determine ds_abs1.ds_abs1_tx.state *)
-val ref_rel_spi_tx_trans_done = store_thm("ref_rel_spi_tx_trans_done",
+(* a lemma to determine ds_abs1.state *)
+(* If spi.state = tx_trans_done, then ds_abs1 is also able to perform TX label transition *)
+val spi_tx_trans_done_imply_abs1_tx_enable = store_thm("spi_tx_trans_done_imply_abs1_tx_enable",
 ``!(spi:spi_state) (dr:driver_state) (ds_abs1:ds_abs1_state).
-(ref_rel ds_abs1 dr spi) /\ (spi.tx.state = tx_trans_done) ==>
+(ref_rel ds_abs1 dr spi) /\ (spi.state = tx_trans_done) ==>
 (ABS1_TX_LBL_ENABLE ds_abs1)``,
 rw [ABS1_TX_LBL_ENABLE_def] >>
-`IS_TX_REL ds_abs1 dr spi` by METIS_TAC[ref_rel_def] >>
-FULL_SIMP_TAC std_ss [IS_TX_REL_def] >>
-Cases_on `dr.dr_tx.state` >>
-rw [] >|
-[`spi.tx.state <> tx_not_ready` by rw [] >>
-`ds_abs1.ds_abs1_tx.state <> abs1_tx_not_ready` by METIS_TAC [] >>
-Cases_on `ds_abs1.ds_abs1_tx.state` >>
-rw [],
-`spi.tx.state <> tx_idle` by rw [] >>
-`ds_abs1.ds_abs1_tx.state <> abs1_tx_pre` by METIS_TAC [] >>
-Cases_on `ds_abs1.ds_abs1_tx.state` >>
-rw [],
-`spi.tx.state <> tx_idle` by rw [] >>
-`ds_abs1.ds_abs1_tx.state <> abs1_tx_idle` by METIS_TAC [] >>
-Cases_on `ds_abs1.ds_abs1_tx.state` >>
-rw [],
-`spi.tx.state <> tx_conf_ready` by rw [] >>
-`ds_abs1.ds_abs1_tx.state <> abs1_tx_idle` by METIS_TAC [] >>
-Cases_on `ds_abs1.ds_abs1_tx.state` >>
-rw [],
-`(spi.tx.state <> tx_trans_check) /\ (spi.tx.state <> tx_ready_for_trans)` by rw [] >>
-`(ds_abs1.ds_abs1_tx.state <> abs1_tx_ready_for_reset) /\
-(ds_abs1.ds_abs1_tx.state <> abs1_tx_reset)` by METIS_TAC [] >>
-Cases_on `ds_abs1.ds_abs1_tx.state` >>
-rw [],
-`spi.tx.state <> tx_channel_disabled` by rw [] >>
-`ds_abs1.ds_abs1_tx.state <> abs1_tx_reset` by METIS_TAC [] >>
-Cases_on `ds_abs1.ds_abs1_tx.state` >>
-rw []]);
+`IS_STATE_REL ds_abs1 dr spi` by METIS_TAC[ref_rel_def] >>
+FULL_SIMP_TAC std_ss [IS_STATE_REL_def] >>
+Cases_on `dr.state` >>
+rw [] >>
+`(spi.state <> init_start) /\
+(spi.state <> init_reset) /\
+(spi.state <> init_setregs) /\
+(spi.state <> spi_ready) /\
+(spi.state <> tx_conf_ready) /\
+(spi.state <> tx_channel_enabled) /\
+(spi.state <> tx_ready_for_trans) /\
+(spi.state <> tx_trans_data) /\
+(spi.state <> tx_channel_disabled) /\
+(spi.state <> rx_conf_ready) /\
+(spi.state <> rx_channel_enabled) /\
+(spi.state <> rx_receive_data) /\
+(spi.state <> rx_update_RX0) /\
+(spi.state <> rx_data_ready) /\
+(spi.state <> rx_channel_disabled) /\
+(spi.state <> xfer_conf_ready) /\
+(spi.state <> xfer_channel_enabled) /\
+(spi.state <> xfer_ready_for_trans) /\
+(spi.state <> xfer_trans_data) /\
+(spi.state <> xfer_exchange_data) /\
+(spi.state <> xfer_update_RX0) /\
+(spi.state <> xfer_data_ready) /\
+(spi.state <> xfer_channel_disabled)` by rw [] >>
+Cases_on `ds_abs1.state` >>
+rw []);
 
 (* bisimulation: ds_abs1' exists for TX label *)
 val abs1_comb_hold_ref_rel_TX = store_thm("abs1_comb_hold_ref_rel_TX",
@@ -48,7 +49,7 @@ val abs1_comb_hold_ref_rel_TX = store_thm("abs1_comb_hold_ref_rel_TX",
 (ref_rel ds_abs1 dr spi) /\ (spi_tr spi (TX data) spi') ==>
 ?ds_abs1'. (ds_abs1_tr ds_abs1 (TX data) ds_abs1') /\ (ref_rel ds_abs1' dr spi')``,
 rw [spi_tr_cases] >>
-`ABS1_TX_LBL_ENABLE ds_abs1` by METIS_TAC[ref_rel_spi_tx_trans_done] >>
+`ABS1_TX_LBL_ENABLE ds_abs1` by METIS_TAC[spi_tx_trans_done_imply_abs1_tx_enable] >>
 rw [ds_abs1_tr_cases] >|
 [(* output data equals *)
 rw [tx_trans_done_op_value_def, tx_trans_done_op_def, 
@@ -58,9 +59,7 @@ METIS_TAC[ref_rel_def, ABS1_TX_LBL_ENABLE_def],
 FULL_SIMP_TAC std_ss [ABS1_TX_LBL_ENABLE_def] >>
 rw [abs1_tx_trans_done_op_state_def, abs1_tx_trans_done_op_def,
 tx_trans_done_op_state_def, tx_trans_done_op_def] >>
-FULL_SIMP_TAC std_ss [ref_rel_def] >>
-rw [] >>
-FULL_SIMP_TAC std_ss [IS_INIT_REL_def, IS_TX_REL_def, IS_RX_REL_def, IS_XFER_REL_def] >>
+FULL_SIMP_TAC std_ss [ref_rel_def, IS_STATE_REL_def] >>
 rw []]);
 
 (* bisimulation: (dr',spi') exists for TX label *)
@@ -70,51 +69,53 @@ val comb_abs1_hold_ref_rel_TX = store_thm("comb_abs1_hold_ref_rel_TX",
 ?dr' spi'. (local_tr (dr, spi) (TX (abs1_tx_trans_done_op_value ds_abs1)) (dr', spi')) /\
 (ref_rel (abs1_tx_trans_done_op_state ds_abs1) dr' spi')``,
 rw [local_tr_cases, spi_tr_cases] >|
-[`spi.tx.state = tx_trans_done` by METIS_TAC[ABS1_TX_LBL_ENABLE_def, ref_rel_def, IS_TX_REL_def] >>
-rw [abs1_tx_trans_done_op_value_def, abs1_tx_trans_done_op_def,
- tx_trans_done_op_value_def, tx_trans_done_op_def] >>
+[`spi.state = tx_trans_done` by METIS_TAC[ABS1_TX_LBL_ENABLE_def, ref_rel_def, IS_STATE_REL_def] >>
+rw [abs1_tx_trans_done_op_value_def, abs1_tx_trans_done_op_def, 
+tx_trans_done_op_value_def, tx_trans_done_op_def] >>
 FULL_SIMP_TAC std_ss [ref_rel_def, ABS1_TX_LBL_ENABLE_def],
-METIS_TAC [ABS1_TX_LBL_ENABLE_def, ref_rel_def, IS_TX_REL_def],
-`spi.tx.state = tx_trans_done` by METIS_TAC[ABS1_TX_LBL_ENABLE_def, ref_rel_def, IS_TX_REL_def] >>
+METIS_TAC [ABS1_TX_LBL_ENABLE_def, ref_rel_def, IS_STATE_REL_def],
+`spi.state = tx_trans_done` by METIS_TAC[ABS1_TX_LBL_ENABLE_def, ref_rel_def, IS_STATE_REL_def] >>
 rw [abs1_tx_trans_done_op_state_def, abs1_tx_trans_done_op_def,
 tx_trans_done_op_state_def, tx_trans_done_op_def] >>
-FULL_SIMP_TAC std_ss [ref_rel_def, ABS1_TX_LBL_ENABLE_def] >>
-rw [] >>
-FULL_SIMP_TAC std_ss [IS_INIT_REL_def, IS_TX_REL_def, IS_RX_REL_def, IS_XFER_REL_def] >>
+FULL_SIMP_TAC std_ss [ref_rel_def, ABS1_TX_LBL_ENABLE_def, IS_STATE_REL_def] >>
 rw []]);
 
-(* a subgoal for bisimulation RX label proof *)
-val ref_rel_spi_rx_receive_data = store_thm("ref_rel_spi_rx_receive_data",
+(* a lemma for RX label proof *)
+(* If spi.state = rx_receive_data, then abs1 is able to process RX label as well. *)
+val spi_rx_receive_data_imply_abs1_rx_enable = store_thm("spi_rx_receive_data_imply_abs1_rx_enable",
 ``!(spi:spi_state) (dr:driver_state) (ds_abs1:ds_abs1_state).
-(ref_rel ds_abs1 dr spi) /\ (spi.rx.state = rx_receive_data) ==>
+(ref_rel ds_abs1 dr spi) /\ (spi.state = rx_receive_data) ==>
 ABS1_RX_LBL_ENABLE ds_abs1``,
 rw [ABS1_RX_LBL_ENABLE_def] >>
-`IS_RX_REL ds_abs1 dr spi` by METIS_TAC[ref_rel_def] >>
-FULL_SIMP_TAC std_ss [IS_RX_REL_def] >>
-Cases_on `dr.dr_rx.state` >>
-rw [] >|
-[`spi.rx.state <> rx_not_ready` by rw [] >>
-`ds_abs1.ds_abs1_rx.state <> abs1_rx_not_ready` by METIS_TAC[] >>
-Cases_on `ds_abs1.ds_abs1_rx.state` >>
-rw[],
-`spi.rx.state <> rx_idle` by rw [] >>
-`ds_abs1.ds_abs1_rx.state <> abs1_rx_pre` by METIS_TAC[] >>
-Cases_on `ds_abs1.ds_abs1_rx.state` >>
-rw[],
-`spi.rx.state <> rx_idle` by rw [] >>
-`ds_abs1.ds_abs1_rx.state <> abs1_rx_idle` by METIS_TAC[] >>
-Cases_on `ds_abs1.ds_abs1_rx.state` >>
-rw[],
-`(spi.rx.state <> rx_conf_ready) ` by rw [] >>
-`ds_abs1.ds_abs1_rx.state <> abs1_rx_idle` by METIS_TAC[] >>
-Cases_on `ds_abs1.ds_abs1_rx.state` >>
-rw[],
-Cases_on `ds_abs1.ds_abs1_rx.state` >>
-rw[],
-`spi.rx.state <> rx_channel_disabled` by rw [] >>
-`ds_abs1.ds_abs1_rx.state <> abs1_rx_reset` by METIS_TAC[] >>
-Cases_on `ds_abs1.ds_abs1_rx.state` >>
-rw[]]);
+`IS_STATE_REL ds_abs1 dr spi` by METIS_TAC[ref_rel_def] >>
+FULL_SIMP_TAC std_ss [IS_STATE_REL_def] >>
+Cases_on `dr.state` >>
+rw [] >>
+`(spi.state <> init_start) /\
+(spi.state <> init_reset) /\
+(spi.state <> init_setregs) /\
+(spi.state <> spi_ready) /\
+(spi.state <> tx_conf_ready) /\
+(spi.state <> tx_channel_enabled) /\
+(spi.state <> tx_ready_for_trans) /\
+(spi.state <> tx_trans_data) /\
+(spi.state <> tx_trans_done) /\
+(spi.state <> tx_channel_disabled) /\
+(spi.state <> rx_conf_ready) /\
+(spi.state <> rx_channel_enabled) /\
+(spi.state <> rx_update_RX0) /\
+(spi.state <> rx_data_ready) /\
+(spi.state <> rx_channel_disabled) /\
+(spi.state <> xfer_conf_ready) /\
+(spi.state <> xfer_channel_enabled) /\
+(spi.state <> xfer_ready_for_trans) /\
+(spi.state <> xfer_trans_data) /\
+(spi.state <> xfer_exchange_data) /\
+(spi.state <> xfer_update_RX0) /\
+(spi.state <> xfer_data_ready) /\
+(spi.state <> xfer_channel_disabled)` by rw [] >>
+Cases_on `ds_abs1.state` >>
+rw []);
 
 
 (* bisimulation: ds_abs1' exists for RX label *)
@@ -123,97 +124,66 @@ val abs1_comb_hold_ref_rel_RX = store_thm("abs1_comb_hold_ref_rel_RX",
 (ref_rel ds_abs1 dr spi) /\ (spi_tr spi (RX data) spi') ==>
 ?ds_abs1'. (ds_abs1_tr ds_abs1 (RX data) ds_abs1') /\ (ref_rel ds_abs1' dr spi')``,
 rw [spi_tr_cases, ds_abs1_tr_cases] >|
-[METIS_TAC [ref_rel_spi_rx_receive_data],
-`ABS1_RX_LBL_ENABLE ds_abs1` by METIS_TAC[ref_rel_spi_rx_receive_data] >>
+[METIS_TAC [spi_rx_receive_data_imply_abs1_rx_enable],
+`ABS1_RX_LBL_ENABLE ds_abs1` by METIS_TAC [spi_rx_receive_data_imply_abs1_rx_enable] >>
 FULL_SIMP_TAC std_ss [ABS1_RX_LBL_ENABLE_def] >>
 rw [abs1_rx_receive_data_op_def, rx_receive_data_op_def, abs1_rx_receive_op_def,
-abs1_rx_done_op_def, abs1_rx_last_op_def] >>
-FULL_SIMP_TAC std_ss [ref_rel_def] >>
-rw [] >>
-FULL_SIMP_TAC std_ss [IS_INIT_REL_def, IS_TX_REL_def, IS_RX_REL_def, IS_XFER_REL_def] >>
+abs1_rx_fetch_data_op_def, abs1_rx_done_op_def] >>
+FULL_SIMP_TAC std_ss [ref_rel_def, IS_STATE_REL_def] >>
 rw []]);
 
 (* bisimulation: (dr',spi') exists for RX label *)
 val comb_abs1_hold_ref_rel_RX = store_thm("comb_abs1_hold_ref_rel_RX",
 ``!(spi:spi_state) (dr:driver_state) (ds_abs1:ds_abs1_state) (data:word8 option).
-(ref_rel ds_abs1 dr spi) /\ (ABS1_RX_LBL_ENABLE ds_abs1) ==>
+(ref_rel ds_abs1 dr spi) /\ (ABS1_RX_LBL_ENABLE ds_abs1) /\
+(data <> NONE) ==>
 ?dr' spi'. local_tr (dr,spi) (RX data) (dr', spi') /\
 (ref_rel (abs1_rx_receive_data_op ds_abs1 data) dr' spi')``,
 rw [local_tr_cases, spi_tr_cases] >|
-[METIS_TAC [ref_rel_def, IS_RX_REL_def, ABS1_RX_LBL_ENABLE_def],
-`spi.rx.state = rx_receive_data` by METIS_TAC[ref_rel_def, IS_RX_REL_def, ABS1_RX_LBL_ENABLE_def] >>
+[METIS_TAC [ref_rel_def, IS_STATE_REL_def, ABS1_RX_LBL_ENABLE_def],
+`spi.state = rx_receive_data` by METIS_TAC[ref_rel_def, IS_STATE_REL_def, ABS1_RX_LBL_ENABLE_def] >>
 FULL_SIMP_TAC std_ss [ABS1_RX_LBL_ENABLE_def] >>
 rw [abs1_rx_receive_data_op_def, abs1_rx_receive_op_def,
-abs1_rx_last_op_def, abs1_rx_done_op_def, rx_receive_data_op_def] >>
-FULL_SIMP_TAC std_ss [ref_rel_def] >>
-rw [] >>
-FULL_SIMP_TAC std_ss [IS_INIT_REL_def, IS_TX_REL_def, IS_RX_REL_def, IS_XFER_REL_def] >>
+abs1_rx_fetch_data_op_def, abs1_rx_done_op_def, rx_receive_data_op_def] >>
+FULL_SIMP_TAC std_ss [ref_rel_def, IS_STATE_REL_def] >>
 rw []]);
 
-(* a subgoal for bisimulation XFER label *)
-val ref_rel_spi_xfer_exchange_data = store_thm("ref_rel_spi_xfer_exchange_data",
+(* a lemma for XFER label *)
+(* If spi.state = xfer_exchange_data, then abs1.state = abs1_xfer_exchange_data *)
+val spi_xfer_exchange_data_imply_abs1_xfer_enable = store_thm("spi_xfer_exchange_data_imply_abs1_xfer_eanble",
 ``!(spi:spi_state) (dr:driver_state) (ds_abs1:ds_abs1_state).
-(ref_rel ds_abs1 dr spi) /\ (spi.xfer.state = xfer_exchange_data) ==>
-ds_abs1.ds_abs1_xfer.state = abs1_xfer_exchange``,
+(ref_rel ds_abs1 dr spi) /\ (spi.state = xfer_exchange_data) ==>
+ds_abs1.state = abs1_xfer_exchange``,
 rw [] >>
-`IS_XFER_REL ds_abs1 dr spi` by METIS_TAC[ref_rel_def] >>
-FULL_SIMP_TAC std_ss [IS_XFER_REL_def] >>
-Cases_on `dr.dr_xfer.state` >>
-rw [] >|
-[`spi.xfer.state <> xfer_not_ready` by rw [] >>
-`ds_abs1.ds_abs1_xfer.state <> abs1_xfer_not_ready` by METIS_TAC[] >>
-Cases_on `ds_abs1.ds_abs1_xfer.state` >>
-rw [],
-`spi.xfer.state <> xfer_idle` by rw [] >>
-`ds_abs1.ds_abs1_xfer.state <> abs1_xfer_pre` by METIS_TAC[] >>
-Cases_on `ds_abs1.ds_abs1_xfer.state` >>
-rw [],
-`spi.xfer.state <> xfer_idle` by rw [] >>
-`ds_abs1.ds_abs1_xfer.state <> abs1_xfer_idle` by METIS_TAC[] >>
-Cases_on `ds_abs1.ds_abs1_xfer.state` >>
-rw [],
-`spi.xfer.state <> xfer_conf_ready` by rw [] >>
-`ds_abs1.ds_abs1_xfer.state <> abs1_xfer_idle` by METIS_TAC[] >>
-Cases_on `ds_abs1.ds_abs1_xfer.state` >>
-rw [],
-`(spi.xfer.state <> xfer_channel_enabled) /\ (spi.xfer.state <> xfer_ready_for_trans) /\
- (spi.xfer.state <> xfer_check)` by rw [] >>
-`(ds_abs1.ds_abs1_xfer.state <> abs1_xfer_idle) /\ 
- (ds_abs1.ds_abs1_xfer.state <> abs1_xfer_prepare) /\
- (ds_abs1.ds_abs1_xfer.state <> abs1_xfer_next)` by METIS_TAC[] >>
-Cases_on `ds_abs1.ds_abs1_xfer.state` >>
-rw [],
-`(spi.xfer.state <> xfer_channel_enabled) /\ (spi.xfer.state <> xfer_ready_for_trans) /\
- (spi.xfer.state <> xfer_check)` by rw [] >>
-`(ds_abs1.ds_abs1_xfer.state <> abs1_xfer_idle) /\ 
- (ds_abs1.ds_abs1_xfer.state <> abs1_xfer_prepare) /\
- (ds_abs1.ds_abs1_xfer.state <> abs1_xfer_next)` by METIS_TAC[] >>
-Cases_on `ds_abs1.ds_abs1_xfer.state` >>
-rw [],
-`(spi.xfer.state <> xfer_ready_for_trans) /\ (spi.xfer.state <> xfer_check)` by rw [] >>
-`(ds_abs1.ds_abs1_xfer.state <> abs1_xfer_trans) /\
- (ds_abs1.ds_abs1_xfer.state <> abs1_xfer_next_write)` by METIS_TAC[] >>
-Cases_on `ds_abs1.ds_abs1_xfer.state` >>
-rw [],
-`spi.xfer.state <> xfer_data_ready` by rw [] >>
-`ds_abs1.ds_abs1_xfer.state <> abs1_xfer_fetch_data` by METIS_TAC[] >>
-Cases_on `ds_abs1.ds_abs1_xfer.state` >>
-rw [],
-`(spi.xfer.state <> xfer_ready_for_trans) /\ (spi.xfer.state <> xfer_check)` by rw [] >>
-`(ds_abs1.ds_abs1_xfer.state <> abs1_xfer_fetch_data) /\
- (ds_abs1.ds_abs1_xfer.state <> abs1_xfer_done)` by METIS_TAC[] >>
-Cases_on `ds_abs1.ds_abs1_xfer.state` >>
-rw [],
-`(spi.xfer.state <> xfer_ready_for_trans) /\ (spi.xfer.state <> xfer_check)` by rw [] >>
-`(ds_abs1.ds_abs1_xfer.state <> abs1_xfer_ready_for_reset) /\
- (ds_abs1.ds_abs1_xfer.state <> abs1_xfer_reset)` by METIS_TAC[] >>
-Cases_on `ds_abs1.ds_abs1_xfer.state` >>
-rw [],
-`spi.xfer.state <> xfer_channel_disabled` by rw [] >>
-`ds_abs1.ds_abs1_xfer.state <> abs1_xfer_reset` by METIS_TAC[] >>
-Cases_on `ds_abs1.ds_abs1_xfer.state` >>
-rw []]);
-
+`IS_STATE_REL ds_abs1 dr spi` by METIS_TAC[ref_rel_def] >>
+FULL_SIMP_TAC std_ss [IS_STATE_REL_def] >>
+Cases_on `dr.state` >>
+rw [] >>
+`(spi.state <> init_start) /\
+(spi.state <> init_reset) /\
+(spi.state <> init_setregs) /\
+(spi.state <> spi_ready) /\
+(spi.state <> tx_conf_ready) /\
+(spi.state <> tx_channel_enabled) /\
+(spi.state <> tx_ready_for_trans) /\
+(spi.state <> tx_trans_data) /\
+(spi.state <> tx_trans_done) /\
+(spi.state <> tx_channel_disabled) /\
+(spi.state <> rx_conf_ready) /\
+(spi.state <> rx_channel_enabled) /\
+(spi.state <> rx_receive_data) /\
+(spi.state <> rx_update_RX0) /\
+(spi.state <> rx_data_ready) /\
+(spi.state <> rx_channel_disabled) /\
+(spi.state <> xfer_conf_ready) /\
+(spi.state <> xfer_channel_enabled) /\
+(spi.state <> xfer_ready_for_trans) /\
+(spi.state <> xfer_trans_data) /\ 
+(spi.state <> xfer_update_RX0) /\
+(spi.state <> xfer_data_ready) /\
+(spi.state <> xfer_channel_disabled)` by rw [] >>
+Cases_on `ds_abs1.state` >>
+rw []);
 
 (* bisimulation: ds_abs1' holds for XFER label *)
 val abs1_comb_hold_ref_rel_XFER = store_thm("abs1_comb_hold_ref_rel_XFER",
@@ -221,7 +191,7 @@ val abs1_comb_hold_ref_rel_XFER = store_thm("abs1_comb_hold_ref_rel_XFER",
 (ref_rel ds_abs1 dr spi) /\ (spi_tr spi (XFER dataIN dataOUT) spi') ==>
 ?ds_abs1'. (ds_abs1_tr ds_abs1 (XFER dataIN dataOUT) ds_abs1') /\ (ref_rel ds_abs1' dr spi')``,
 rw [spi_tr_cases] >>
-`ds_abs1.ds_abs1_xfer.state = abs1_xfer_exchange` by METIS_TAC[ref_rel_spi_xfer_exchange_data] >>
+`ds_abs1.state = abs1_xfer_exchange` by METIS_TAC[spi_xfer_exchange_data_imply_abs1_xfer_enable] >>
 rw [ds_abs1_tr_cases] >|
 [(* output data equals *)
 rw [xfer_exchange_data_op_value_def, xfer_exchange_data_op_def,
@@ -230,30 +200,27 @@ METIS_TAC[ref_rel_def],
 (* ref_rel holds *)
 rw [xfer_exchange_data_op_state_def, xfer_exchange_data_op_def,
 abs1_xfer_exchange_op_state_def, abs1_xfer_exchange_op_def] >>
-FULL_SIMP_TAC std_ss [ref_rel_def] >>
-rw [] >>
-FULL_SIMP_TAC std_ss [IS_INIT_REL_def, IS_TX_REL_def, IS_RX_REL_def, IS_XFER_REL_def] >>
+FULL_SIMP_TAC std_ss [ref_rel_def, IS_STATE_REL_def] >>
 rw []]);
 
 (* bisimulation: (dr',spi') exists for XFER label *)
 val comb_abs1_hold_ref_rel_XFER = store_thm("comb_abs1_hold_ref_rel_XFER",
 ``!(spi:spi_state) (dr:driver_state) (ds_abs1:ds_abs1_state) (dataIN:word8 option).
-(ref_rel ds_abs1 dr spi) /\ (ds_abs1.ds_abs1_xfer.state = abs1_xfer_exchange) ==>
+(ref_rel ds_abs1 dr spi) /\ (ds_abs1.state = abs1_xfer_exchange) /\
+(dataIN <> NONE) ==>
 ?dr' spi'. (local_tr (dr, spi) (XFER dataIN (abs1_xfer_exchange_op_value 
 ds_abs1 dataIN)) (dr', spi')) /\ 
 (ref_rel (abs1_xfer_exchange_op_state ds_abs1 dataIN) dr' spi')``,
 rw [local_tr_cases, spi_tr_cases] >|
-[`spi.xfer.state = xfer_exchange_data` by METIS_TAC[ref_rel_def, IS_XFER_REL_def] >>
+[`spi.state = xfer_exchange_data` by METIS_TAC[ref_rel_def, IS_STATE_REL_def] >>
 rw [abs1_xfer_exchange_op_value_def, abs1_xfer_exchange_op_def,
 xfer_exchange_data_op_value_def, xfer_exchange_data_op_def] >>
 FULL_SIMP_TAC std_ss [ref_rel_def],
-METIS_TAC [ref_rel_def, IS_XFER_REL_def],
-`spi.xfer.state = xfer_exchange_data` by METIS_TAC[ref_rel_def, IS_XFER_REL_def] >>
+METIS_TAC [ref_rel_def, IS_STATE_REL_def],
+`spi.state = xfer_exchange_data` by METIS_TAC[ref_rel_def, IS_STATE_REL_def] >>
 rw [abs1_xfer_exchange_op_state_def, abs1_xfer_exchange_op_def,
 xfer_exchange_data_op_state_def, xfer_exchange_data_op_def] >>
-FULL_SIMP_TAC std_ss [ref_rel_def] >>
-rw [] >>
-FULL_SIMP_TAC std_ss [IS_INIT_REL_def, IS_TX_REL_def, IS_RX_REL_def, IS_XFER_REL_def] >>
+FULL_SIMP_TAC std_ss [ref_rel_def, IS_STATE_REL_def] >>
 rw []]);
 
 val _ = export_theory();
